theories/L2k_noCnstrParams/stripEvalCommute.v
@@ -8,7 +8,10 @@ Require Import Coq.Setoids.Setoid.
 Require Import Coq.micromega.Lia.
 
 Require Import Common.Common.
-Require Import L1g.L1g.
+
+From MetaCoq.Template Require Import BasicAst Ast.
+From MetaCoq.Erasure Require Import EAst EAstUtils.
+
 Require Import L2k.compile.
 Require Import L2k.term.
 Require Import L2k.program.
@@ -18,117 +21,157 @@ Local Open Scope string_scope.
 Local Open Scope bool.
 Local Open Scope list.
 Set Implicit Arguments.
-(* 
-Definition L2dTerm := L1g.compile.Term.
-Definition L2dTerms := L1g.compile.Terms.
-Definition L2dBrs := L1g.compile.Brs.
-Definition L2dDefs := L1g.compile.Defs.
 
-Notation strips := (strips strip).
+Definition L2dTerm := EAst.term.
+Definition L2dTerms := list EAst.term.
+Definition L2dBrs := list (branch EAst.term).
+Definition L2dDefs := list (def EAst.term).
 
-Definition optStrip (t:option L2dTerm) : option Term :=
+From MetaCoq.Erasure Require Import ESpineView EWcbvEvalEtaInd EWellformed EEtaExpanded.
+
+Definition term_flags :=
+  {|
+    has_tBox := true;
+    has_tRel := true;
+    has_tVar := false;
+    has_tEvar := false;
+    has_tLambda := true;
+    has_tLetIn := true;
+    has_tApp := true;
+    has_tConst := true;
+    has_tConstruct := true;
+    has_tCase := true;
+    has_tProj := true;
+    has_tFix := true;
+    has_tCoFix := false
+  |}.
+
+Definition env_flags := 
+  {| has_axioms := false;
+    has_cstr_params := false;
+    term_switches := term_flags |}.
+
+Local Existing Instance env_flags.
+
+Section OnGlobalEnv.
+  Context (Σ : global_context).
+
+  Notation compile := (compile Σ).
+
+  Definition compile_terms ts := list_terms (map compile ts).
+  
+  Definition compile_br (br : list name * EAst.term) :=
+    (List.rev (fst br), compile (snd br)).
+
+  Definition compile_brs ts := list_Brs (map compile_br ts).
+
+  Definition compile_def d :=
+    {| dname := dname d; dbody := compile d.(dbody); rarg := d.(rarg) |}.
+
+  Definition compile_defs ts := list_Defs (map compile_def ts).
+
+Definition optcompile (t:option L2dTerm) : option Term :=
   match t with
     | None => None
-    | Some t => Some (strip t)
+    | Some t => Some (compile t)
   end.
-Definition optStrips (ts:option L2dTerms) : option Terms :=
+Definition optcompile_terms (ts:option L2dTerms) : option Terms :=
   match ts with
     | None => None
-    | Some ts => Some (strips ts)
+    | Some ts => Some (compile_terms ts)
   end.
-Definition optStripDnth (b: option L2dTerm): option Term :=
+Definition optcompileDnth (b: option L2dTerm): option Term :=
                            match b with
                              | None => None
-                             | Some t => Some (strip t)
+                             | Some t => Some (compile t)
                            end.
-Definition optStripCanP
+Definition optcompileCanP
            (b: option (nat * L2dTerms * nat)): option (nat * Terms * nat) :=
                            match b with
                              | None => None
-                             | Some (n, t, m) => Some (n, strips t, m)
+                             | Some (n, t, m) => Some (n, compile_terms t, m)
                            end.
 (**********************
-Definition optStrip_split
+Definition optcompile_split
            (b: option L2d.term.split): option split :=
   match b with
     | None => None
     | Some (L2d.term.mkSplit fsts t lsts) =>
-      Some (mkSplit (strips fsts) (strip t) (strips lsts))
+      Some (mkSplit (compile_terms fsts) (compile t) (compile_terms lsts))
   end.
 ******************)
 
-Lemma optStrip_hom: forall y, optStrip (Some y) = Some (strip y).
+Lemma optcompile_hom: forall y, optcompile (Some y) = Some (compile y).
 induction y; simpl; reflexivity.
 Qed.
-Lemma optStrip_hom_None: optStrip (@None L2dTerm) = @None (Term).
+Lemma optcompile_hom_None: optcompile (@None L2dTerm) = @None (Term).
   reflexivity.
 Qed.
 
-Lemma optStrips_hom: forall y, optStrips (Some y) = Some (strips y).
+Lemma optcompile_terms_hom: forall y, optcompile_terms (Some y) = Some (compile_terms y).
 induction y; simpl; reflexivity.
 Qed.
-Lemma optStripDnth_hom:
-  forall y, optStripDnth (Some y) = Some (strip y).
+Lemma optcompileDnth_hom:
+  forall y, optcompileDnth (Some y) = Some (compile y).
 induction y; simpl; reflexivity.
 Qed.
-Lemma optStripCanP_hom:
-  forall y n m, optStripCanP (Some (n, y, m)) = Some (n, strips y, m).
+Lemma optcompileCanP_hom:
+  forall y n m, optcompileCanP (Some (n, y, m)) = Some (n, compile_terms y, m).
 induction y; simpl; reflexivity.
 Qed.
 (*********************
-Lemma optStrip_split_hom:
+Lemma optcompile_split_hom:
   forall fsts t lsts,
-    optStrip_split (Some (L2d.term.mkSplit fsts t lsts)) =
-    Some (mkSplit (strips fsts) (strip t) (strips lsts)).
+    optcompile_split (Some (L2d.term.mkSplit fsts t lsts)) =
+    Some (mkSplit (compile_terms fsts) (compile t) (compile_terms lsts)).
 Proof.
   induction fsts; cbn; intros; try reflexivity.
 Qed.
  ***********************)
 
 Lemma tlength_hom:
-  forall ts, tlength (strips ts) = List.length ts.
+  forall ts, tlength (compile_terms ts) = List.length ts.
 Proof.
   induction ts; intros; try reflexivity.
   - cbn. apply f_equal. assumption.
 Qed.
-  
-Lemma Lookup_hom:
-  forall p s ec, Lookup s p ec -> Lookup s (stripEnv p) (stripEC ec).
-Proof.
-  induction 1; destruct t.
-  - change (Lookup s ((s, ecTrm (strip l)) :: (stripEnv p))
-                   (ecTrm (strip l))).
-    apply LHit.
-  - cbn. apply LHit.
-  - change (Lookup s2 ((s1, ecTrm (strip l)) :: (stripEnv p))
-                   (stripEC ec)).
-    apply LMiss; assumption.
-  - cbn. apply LMiss; assumption.
-Qed.
 
-Lemma lookup_hom:
-  forall p nm ec,
-    lookup nm p = Some ec -> lookup nm (stripEnv p) = Some (stripEC ec).
+From Coq Require Import ssreflect.
+From MetaCoq.Template Require Import utils.
+From MetaCoq.Erasure Require Import EGlobalEnv EExtends.
+
+Lemma Lookup_hom:
+  forall s ec, lookup_env Σ s = Some ec -> 
+    ∑ Σ', extends Σ' Σ × lookup s (compile_ctx Σ) = Some (compile_global_decl Σ' ec).
 Proof.
-  intros p nm ec h. apply Lookup_lookup.
-  apply Lookup_hom. apply (lookup_Lookup _ _ h).
+  induction Σ; cbn => //.
+  intros s ec.
+  case: eqb_specT.
+  - intros -> [= <-].
+    exists g. split. now exists [a].
+    destruct a as [kn d]; cbn.
+    now rewrite eqb_refl.
+  - intros neq hl.
+    destruct (IHg _ _ hl) as [Σ' [ext hl']].
+    exists Σ'. split.
+    destruct ext as [Σ'' ->]. now exists (a :: Σ'').
+    destruct a as [kn d]; cbn.
+    cbn in neq; case: eqb_specT => //.
 Qed.
   
 Lemma lookup_hom_None:
-  forall p nm,
-    lookup nm p = None -> lookup nm (stripEnv p) = None.
+  forall nm,
+    lookup_env Σ nm = None -> lookup nm (compile_ctx Σ) = None.
 Proof.
-  induction p; intros.
+  induction Σ; intros.
   - cbn. reflexivity.
-  - destruct a. destruct (kername_eq_dec nm k).
-    + subst. cbn in H. rewrite eq_kername_refl in H. discriminate.
-    + cbn. rewrite (eq_kername_bool_neq n).
-      cbn in H. rewrite (eq_kername_bool_neq n) in H.
-      apply IHp. assumption.
+  - destruct a. cbn in *.
+    destruct (eqb_spec nm k) => //.
+    now apply IHg.
 Qed.
   
-Lemma LookupDfn_hom:
-  forall p s t, LookupDfn s p t -> LookupDfn s (stripEnv p) (strip t).
+(*Lemma LookupDfn_hom:
+  forall p s t, LookupDfn s p t -> LookupDfn s (compile_ctx Σ) (compile t).
 Proof.
   unfold LookupDfn. intros.
   assert (j:= Lookup_hom H). exact j.
@@ -136,7 +179,7 @@ Qed.
 
 Lemma lookupDfn_hom:
   forall p nm t,
-    lookupDfn nm p = Ret t -> lookupDfn nm (stripEnv p) = Ret (strip t).
+    lookupDfn nm p = Ret t -> lookupDfn nm (compile_ctx Σ) = Ret (compile t).
 Proof.
   induction p; intros.
   - cbn in *. discriminate.
@@ -151,73 +194,74 @@ Proof.
       * rewrite (lookup_hom _ _ H0). destruct e0; try discriminate.
         cbn. myInjection H. reflexivity.
 Qed.
+*)
 
 Lemma dlength_hom:
-  forall ds, L1g.compile.dlength ds = dlength (stripDs ds).
+  forall ds, List.length ds = dlength (compile_defs ds).
 induction ds. intuition. simpl. rewrite IHds. reflexivity.
 Qed.
 
 Lemma tcons_hom:
-  forall t ts, strips (cons t ts) = tcons (strip t) (strips ts).
+  forall t ts, compile_terms (cons t ts) = tcons (compile t) (compile_terms ts).
 reflexivity.
 Qed.
 
-Lemma tnil_hom: strips nil = tnil.
+Lemma tnil_hom: compile_terms nil = tnil.
 reflexivity.
 Qed.
-
+(* 
 Lemma dcons_hom:
   forall nm bod rarg ds,
-    stripDs (L1g.compile.dcons nm bod rarg ds) =
-    dcons nm (strip bod) rarg (stripDs ds).
+    compile_defs (L1g.compile.dcons nm bod rarg ds) =
+    dcons nm (compile bod) rarg (compile_defs ds).
 reflexivity.
-Qed.
-
-Lemma dnil_hom: stripDs L1g.compile.dnil = dnil.
+Qed. *)
+(* 
+Lemma dnil_hom: compile_defs L1g.compile.dnil = dnil.
 reflexivity.
-Qed.
-
+Qed. *)
+(* 
 Lemma dnthBody_hom: 
-  forall m ds, optStripDnth (option_map fst (L1g.compile.dnthBody m ds)) =
-               dnthBody m (stripDs ds).
+  forall m ds, optcompileDnth (option_map fst (L1g.compile.dnthBody m ds)) =
+               dnthBody m (compile_defs ds).
 induction m; induction ds; try intuition auto.
 - simpl. unfold dnthBody. simpl. apply IHm.
-Qed.
+Qed. *)
 
 Lemma tnth_hom:
- forall ts n, optStrip (List.nth_error ts n) = tnth n (strips ts).
+ forall ts n, optcompile (List.nth_error ts n) = tnth n (compile_terms ts).
 induction ts; simpl; intros n; case n; try reflexivity; trivial.
 Qed. 
 
 (* Lemma tskipn_hom: *)
-(*   forall ts n, optStrips (List.skipn n ts) = tskipn n (strips ts). *)
+(*   forall ts n, optcompile_terms (List.skipn n ts) = tskipn n (compile_terms ts). *)
 (* induction ts; simpl; intros n; case n; try reflexivity; trivial. *)
 (* Qed. *)
 
 Lemma tappend_hom:
-  forall ts us : list L1gTerm,
-    strips (List.app ts us) = tappend (strips ts) (strips us).
+  forall ts us : list EAst.term,
+    compile_terms (List.app ts us) = tappend (compile_terms ts) (compile_terms us).
 Proof.
   induction ts; intros us; simpl. reflexivity.
-  rewrite IHts. reflexivity.
+  cbn. f_equal. apply IHts.
 Qed.
 
-Lemma TApp_hom:
+(* Lemma TApp_hom:
   forall fn arg,
-    strip (L1g.compile.TApp fn arg) =
-    match CanonicalP strip fn (strip arg) with
-    | None => TApp (strip fn) (strip arg)
+    compile (TApp fn arg) =
+    match CanonicalP compile fn (compile arg) with
+    | None => TApp (compile fn) (compile arg)
     | Some (F, args, npars, nargs) => etaExpand F args npars nargs
     end.
 Proof.
   reflexivity.
-Qed.
+Qed. *)
 
 (***
 Lemma TAppCnstr_hom:
   forall i m npars nargs arg args, 
-    strip (L2d.compile.TApp (L2d.compile.TConstruct i m npars nargs) arg args) =
-    etaExpand i m npars nargs (tcons (strip arg) (strips args)).
+    compile (L2d.compile.TApp (L2d.compile.TConstruct i m npars nargs) arg args) =
+    etaExpand i m npars nargs (tcons (compile arg) (compile_terms args)).
 Proof.
   intros. reflexivity.
 Qed.
@@ -280,13 +324,13 @@ Qed.
   
 
 Lemma isApp_hom:
-  forall t, isApp (strip t) -> L2d.term.isApp t.
+  forall t, isApp (compile t) -> L2d.term.isApp t.
 Proof.
 Admitted.
 (************
   destruct t; intros h; destruct h as [x0 [x1 jx]]; try discriminate.
   - auto.
-  - unfold strip in jx. 
+  - unfold compile in jx. 
     elim (notIsApp_etaExpand i n tnil n0 n1). rewrite jx. auto.
 Qed.
  *****************)   
@@ -317,10 +361,10 @@ Qed.
 (*************
 Lemma isLambda_hom:
   forall t,
-    isLambda (strip t) ->
+    isLambda (compile t) ->
     L2d.term.isLambda t \/ L2d.term.isConstruct t \/  L2d.term.isApp t.
 Proof.
-  intros t. functional induction (strip t); intros h;
+  intros t. functional induction (compile t); intros h;
   destruct h as [x0 [x1 jx]]; try discriminate.
   - left. auto.
   - right. right. auto.
@@ -328,12 +372,12 @@ Proof.
 Qed.
 
 Lemma isFix_hom:
-  forall t, isFix (strip t) -> L2d.term.isFix t.
+  forall t, isFix (compile t) -> L2d.term.isFix t.
 Proof.
   induction t; intros; simpl in *;
   try (destruct H as [x0 [x1 jx]]; discriminate); auto.
   - destruct t1; try (destruct H as [x0 [x1 jx]]; discriminate).
-    destruct (etaExp_cnstr_Sanity' i n n0 n1 (tcons (strip t2) (strips t3))).
+    destruct (etaExp_cnstr_Sanity' i n n0 n1 (tcons (compile t2) (compile_terms t3))).
     + rewrite H0 in H. destruct H as [x0 [x1 jx]]. discriminate.
     + rewrite H0 in H. destruct H as [x0 [x1 jx]]. discriminate.
   - destruct (etaExp_cnstr_Sanity' i n n0 n1 tnil).
@@ -343,20 +387,20 @@ Proof.
 Qed.
 
 Lemma L2WFapp_L2kWFapp:
-  (forall t, L2d.term.WFapp t -> WFapp (strip t)) /\
-  (forall ts, L2d.term.WFapps ts -> WFapps (strips ts)) /\
-  (forall ts, L2d.term.WFappBs ts -> WFappBs (stripBs ts)) /\
-  (forall ds, L2d.term.WFappDs ds -> WFappDs (stripDs ds)).
+  (forall t, L2d.term.WFapp t -> WFapp (compile t)) /\
+  (forall ts, L2d.term.WFapps ts -> WFapps (compile_terms ts)) /\
+  (forall ts, L2d.term.WFappBs ts -> WFappBs (compileBs ts)) /\
+  (forall ds, L2d.term.WFappDs ds -> WFappDs (compile_defs ds)).
 Proof.
   apply L2d.term.WFappTrmsBrsDefs_ind; try constructor; auto; intros.
   - destruct fn; auto; try (constructor; try assumption; not_isApp).
     + elim H. auto.
     + change
-        (WFapp (match nat_compare (n0 + n1) (S (tlength (strips ts))) with
+        (WFapp (match nat_compare (n0 + n1) (S (tlength (compile_terms ts))) with
         | Lt => TWrong
-        | _ => etaExp_cnstr i n n0 n1 (tcons (strip t) (strips ts))
+        | _ => etaExp_cnstr i n n0 n1 (tcons (compile t) (compile_terms ts))
         end)).
-      destruct (n0 + n1 ?= S (tlength (strips ts))).
+      destruct (n0 + n1 ?= S (tlength (compile_terms ts))).
       
     + apply etaExp_cnstr_pres_WFapp. constructor; assumption.
     + destruct p. constructor; try assumption. not_isApp.
@@ -365,21 +409,21 @@ Proof.
 Qed.
 
 Lemma L2WFaEnv_L2kWFaEnv:
-  forall p:environ L2Term, L2d.program.WFaEnv p -> WFaEnv (stripEnv p).
+  forall p:environ L2Term, L2d.program.WFaEnv p -> WFaEnv (compile_ctx Σ).
 Proof.
   induction 1; simpl; constructor.
   - inversion H; destruct ec; simpl; try discriminate; constructor.
     + apply (proj1 (L2WFapp_L2kWFapp)). assumption.
   - assumption.
-  - apply stripEnv_pres_fresh. assumption.
+  - apply compile_ctx_pres_fresh. assumption.
 Qed.
  ************)
 
 (***
 Lemma WFapp_hom:
-  (forall t, L2d.term.WFapp t -> WFapp (strip t)) /\
-  (forall ts, L2d.term.WFapps ts -> WFapps (strips ts)) /\
-  (forall ds, L2d.term.WFappDs ds -> WFappDs (stripDs ds)).
+  (forall t, L2d.term.WFapp t -> WFapp (compile t)) /\
+  (forall ts, L2d.term.WFapps ts -> WFapps (compile_terms ts)) /\
+  (forall ds, L2d.term.WFappDs ds -> WFappDs (compile_defs ds)).
 Proof.
    apply L2d.term.WFappTrmsDefs_ind; cbn; intros;
   try (solve [constructor]);
@@ -388,14 +432,14 @@ Proof.
     + intros h. assert (j:= isApp_hom _ h). contradiction.
 Qed.
  ****)
-
+(* 
 Lemma mkApp_tcons_lem1:
   forall fn arg args,
     L1g.compile.mkApp (L1g.compile.mkApp fn (cons arg args)) nil = L1g.compile.mkApp fn (cons arg args).
 Proof.
   destruct fn; intros arg args; simpl;
   try rewrite tappend_tnil; try reflexivity.
-Qed.
+Qed. *)
 
 (**********
 Lemma mkApp_tcons_lem2:
@@ -585,10 +629,10 @@ Qed.
  **************)
 
 (**********
-Lemma strip_App_not_Constructor:
+Lemma compile_App_not_Constructor:
   forall fn arg,
     ~ L2d.term.isConstruct fn ->
-    strip (L2d.compile.TApp fn arg) = TApp (strip fn) (strip arg).
+    compile (L2d.compile.TApp fn arg) = TApp (compile fn) (compile arg).
 Proof.
   intros. case_eq fn; intros; subst; try reflexivity.
   elim H; auto.
@@ -602,13 +646,18 @@ Definition notApp (F:Terms -> Term) :=
 
 Lemma isApp_fn_not_isConstruct:
   forall fn arg,
-    isApp (strip (L1g.compile.TApp fn arg)) -> ~ L1g.term.isConstruct fn.
+    isApp (compile (tApp fn arg)) -> ~ EAstUtils.isConstruct fn.
 Proof.
 Admitted.
+
+
+
+
+
 (*******************
   intros. intro h. destruct h as [x0 [x1 [x2 [x3 jx]]]]. subst fn.
   change
-    (isApp (etaExpand x0 x1 (strips (L2d.compile.tunit arg)) x2 x3)) in H.
+    (isApp (etaExpand x0 x1 (compile_terms (L2d.compile.tunit arg)) x2 x3)) in H.
   eelim notIsApp_etaExpand. eassumption.
 Qed.
  *******************)
@@ -618,7 +667,7 @@ Lemma mkApp_hom:
   forall fn args,
     ~ L2d.term.isApp fn ->
     ~ L2d.term.isConstruct fn ->
-    strip (L2d.term.mkApp fn args) = mkApp (strip fn) (strips args).
+    compile (L2d.term.mkApp fn args) = mkApp (compile fn) (compile_terms args).
 Proof.
   intros fn. destruct (L2d.term.isConstruct_dec fn);
   induction args; intros.
@@ -633,7 +682,7 @@ Proof.
     Lemma mkApp_hom:
   forall fn args,
     ~ L2d.term.isApp fn ->
-    strip (L2d.term.mkApp fn args) = mkApp (strip fn) (strips args).
+    compile (L2d.term.mkApp fn args) = mkApp (compile fn) (compile_terms args).
 Proof.
   intros fn. destruct (L2d.term.isConstruct_dec fn);
   induction args; intros.
@@ -641,14 +690,14 @@ Proof.
   - destruct i as [x0 [x1 [x2 [x3 jx]]]]. subst.
     rewrite L2d.term.mkApp_goodFn.
     change
-      (etaExpand x0 x1 (tcons (strip t) (strips args)) x2 x3 =
+      (etaExpand x0 x1 (tcons (compile t) (compile_terms args)) x2 x3 =
        mkApp (etaExpand x0 x1 tnil x2 x3)
-             (strips (L2d.compile.tcons t args))).
+             (compile_terms (L2d.compile.tcons t args))).
     specialize (IHargs H H0).
     change
-      (strip (L2d.term.mkApp (L2d.compile.TConstruct x0 x1 x2 x3) args) =
+      (compile (L2d.term.mkApp (L2d.compile.TConstruct x0 x1 x2 x3) args) =
        mkApp (etaExpand x0 x1 tnil x2 x3)
-             (strips args)) in IHargs.
+             (compile_terms args)) in IHargs.
     rewrite tcons_hom. rewrite mkApp_goodFn.
     case_eq args; intros.
     + rewrite tnil_hom. 
@@ -663,7 +712,7 @@ Lemma mkApp_hom:
   forall args fn,
     ~ L2d.term.isApp fn ->
     ~ L2d.term.isConstruct fn ->
-    strip (L2d.term.mkApp fn args) = mkApp (strip fn) (strips args).
+    compile (L2d.term.mkApp fn args) = mkApp (compile fn) (compile_terms args).
 Proof.
   induction args; intros.
   - rewrite mkApp_tnil_ident. rewrite L2d.term.mkApp_tnil_ident. reflexivity.
@@ -677,17 +726,17 @@ Qed.
 (*****************
 Lemma instantiate_hom:
   (forall bod n, L2d.term.WFTrm bod n -> 
-                 forall arg, strip (L2d.term.instantiate arg n bod) =
-                             instantiate (strip arg) n (strip bod)) /\
+                 forall arg, compile (L2d.term.instantiate arg n bod) =
+                             instantiate (compile arg) n (compile bod)) /\
   (forall bods n, L2d.term.WFTrms bods n ->
-                  forall arg, strips (L2d.term.instantiates arg n bods) =
-                              instantiates (strip arg) n (strips bods)) /\
+                  forall arg, compile_terms (L2d.term.instantiates arg n bods) =
+                              instantiates (compile arg) n (compile_terms bods)) /\
   (forall bods n, L2d.term.WFTrmBs bods n ->
-                  forall arg, stripBs (L2d.term.instantiateBrs arg n bods) =
-                              instantiateBrs (strip arg) n (stripBs bods)) /\
+                  forall arg, compileBs (L2d.term.instantiateBrs arg n bods) =
+                              instantiateBrs (compile arg) n (compileBs bods)) /\
   (forall ds n, L2d.term.WFTrmDs ds n  ->
-                forall arg, stripDs (L2d.term.instantiateDefs arg n ds) =
-                            instantiateDefs (strip arg) n (stripDs ds)).
+                forall arg, compile_defs (L2d.term.instantiateDefs arg n ds) =
+                            instantiateDefs (compile arg) n (compile_defs ds)).
 Proof.
   apply L2d.term.WFTrmTrmsBrsDefs_ind; intros;
     try (cbn; reflexivity); try (cbn; rewrite H0; reflexivity).
@@ -696,51 +745,51 @@ Proof.
   - destruct (L2d.term.isConstruct_dec fn).
     + destruct i as [x0 [x1 [x2 [x3 jx]]]]. subst.
       change
-        (strip
+        (compile
            (L2d.term.instantiate
               arg n (L2d.compile.TApp
                        (L2d.compile.TConstruct x0 x1 x2 x3) t ts)) =
-         instantiate (strip arg) n
-                     (strip (L2d.compile.TApp
+         instantiate (compile arg) n
+                     (compile (L2d.compile.TApp
                                (L2d.compile.TConstruct x0 x1 x2 x3) t ts))).
       change
-        (strip
+        (compile
            (L2d.term.mkApp
               (L2d.term.instantiate
                  arg n (L2d.compile.TConstruct x0 x1 x2 x3))
               (L2d.term.instantiates arg n (L2d.compile.tcons t ts))) =
-         instantiate (strip arg) n
-                     (strip (L2d.compile.TApp
+         instantiate (compile arg) n
+                     (compile (L2d.compile.TApp
                                (L2d.compile.TConstruct x0 x1 x2 x3) t ts))).
       rewrite mkApp_hom.
       
       
       change
-        (strip (L2d.compile.TApp (L2d.compile.TConstruct x0 x1 x2 x3)
+        (compile (L2d.compile.TApp (L2d.compile.TConstruct x0 x1 x2 x3)
                                 (L2d.term.instantiate arg n t)
                                 (L2d.term.instantiates arg n ts)) =
          instantiate
-           (strip arg)
-           n (etaExpand x0 x1 (tcons (strip t) (strips ts)) x2 x3)).
+           (compile arg)
+           n (etaExpand x0 x1 (tcons (compile t) (compile_terms ts)) x2 x3)).
       change
-        (etaExpand x0 x1 (tcons (strip (L2d.term.instantiate arg n t))
-                                (strips (L2d.term.instantiates arg n ts)))
+        (etaExpand x0 x1 (tcons (compile (L2d.term.instantiate arg n t))
+                                (compile_terms (L2d.term.instantiates arg n ts)))
                                 x2 x3 =
          instantiate
-           (strip arg)
-           n (etaExpand x0 x1 (tcons (strip t) (strips ts)) x2 x3)).
+           (compile arg)
+           n (etaExpand x0 x1 (tcons (compile t) (compile_terms ts)) x2 x3)).
       rewrite H3. rewrite H5.
 
       admit.
-    + rewrite strip_App_not_Constructor; try assumption.
+    + rewrite compile_App_not_Constructor; try assumption.
       change
-        (strip (L2d.term.mkApp
+        (compile (L2d.term.mkApp
                   (L2d.term.instantiate arg n fn)
                   (L2d.compile.tcons (L2d.term.instantiate arg n t)
                                     (L2d.term.instantiates arg n ts))) =
-         (mkApp (instantiate (strip arg) n (strip fn))
-                (tcons (instantiate (strip arg) n (strip t))
-                       (instantiates (strip arg) n (strips ts))))).
+         (mkApp (instantiate (compile arg) n (compile fn))
+                (tcons (instantiate (compile arg) n (compile t))
+                       (instantiates (compile arg) n (compile_terms ts))))).
       rewrite <- H1. rewrite <- H3. rewrite <- H5.
       rewrite mkApp_hom.
       * rewrite tcons_hom. reflexivity.
@@ -771,20 +820,20 @@ Proof.
         Check (instantiate_pres_shape).
         
     * change
-        (strip (L2d.term.mkApp (L2d.term.instantiate arg n fn)
+        (compile (L2d.term.mkApp (L2d.term.instantiate arg n fn)
                               (L2d.compile.tcons
                                  (L2d.term.instantiate arg n t)
 
                                  (L2d.term.instantiates arg n ts))) =
-         instantiate (strip arg) n (TApp (strip fn) (strip t) (strips ts))).
+         instantiate (compile arg) n (TApp (compile fn) (compile t) (compile_terms ts))).
       change
-        (strip (L2d.term.mkApp (L2d.term.instantiate arg n fn)
+        (compile (L2d.term.mkApp (L2d.term.instantiate arg n fn)
                               (L2d.compile.tcons
                                  (L2d.term.instantiate arg n t)
                                  (L2d.term.instantiates arg n ts))) =
-         mkApp (instantiate (strip arg) n (strip fn))
-               (tcons (instantiate (strip arg) n (strip t))
-                      (instantiates (strip arg) n (strips ts)))).
+         mkApp (instantiate (compile arg) n (compile fn))
+               (tcons (instantiate (compile arg) n (compile t))
+                      (instantiates (compile arg) n (compile_terms ts)))).
       destruct (L2d.term.isApp_dec (L2d.term.instantiate arg n fn)).
       * Check mkApp_hom.
 
@@ -793,18 +842,18 @@ Proof.
 
       * destruct i as [x0 [x1 [x2 jx]]]. rewrite jx.
         change
-          (strip
+          (compile
              (L2d.compile.TApp
                 x0 x1 (L2d.term.tappend
                          x2 (L2d.compile.tcons
                                (L2d.term.instantiate arg n t)
                                (L2d.term.instantiates arg n ts)))) =
-            mkApp (instantiate (strip arg) n (strip fn))
-                  (tcons (instantiate (strip arg) n (strip t))
-                         (instantiates (strip arg) n (strips ts)))).
+            mkApp (instantiate (compile arg) n (compile fn))
+                  (tcons (instantiate (compile arg) n (compile t))
+                         (instantiates (compile arg) n (compile_terms ts)))).
 
         
-        assert (instantiate (strip arg) n (strip fn) = )
+        assert (instantiate (compile arg) n (compile fn) = )
       * rewrite <- instantiate_mkApp_commute.
         rewrite (L2d.term.mkApp_goodFn _ _ n1).
 
@@ -817,31 +866,31 @@ Proof.
     
   - rewrite L2d.term.instantiate_TApp_mkApp.
     change
-      (strip (L2d.term.mkApp (L2d.term.instantiate arg n fn)
+      (compile (L2d.term.mkApp (L2d.term.instantiate arg n fn)
                             (L2d.compile.tcons
                                (L2d.term.instantiate arg n t)
                                (L2d.term.instantiates arg n ts))) =
-       instantiate (strip arg) n (strip (L2d.compile.TApp fn t ts))).
+       instantiate (compile arg) n (compile (L2d.compile.TApp fn t ts))).
     destruct (L2d.term.isConstruct_dec fn).
     + destruct i as [x0 [x1 [x2 [x3 jx]]]]. subst.
       rewrite L2d.term.mkApp_goodFn; try not_isApp.
       unfold L2d.term.instantiate at 1.
       change
         (etaExpand (TConstruct x0 x1)
-                   (tcons (strip (L2d.term.instantiate arg n t))
-                          (strips (L2d.term.instantiates arg n ts)))
+                   (tcons (compile (L2d.term.instantiate arg n t))
+                          (compile_terms (L2d.term.instantiates arg n ts)))
                    x2 x3 =
-         instantiate (strip arg) n
-                     (strip (L2d.compile.TApp
+         instantiate (compile arg) n
+                     (compile (L2d.compile.TApp
                                (L2d.compile.TConstruct x0 x1 x2 x3) t ts))).
       change
         (etaExpand (TConstruct x0 x1)
-                   (tcons (strip (L2d.term.instantiate arg n t))
-                          (strips (L2d.term.instantiates arg n ts)))
+                   (tcons (compile (L2d.term.instantiate arg n t))
+                          (compile_terms (L2d.term.instantiates arg n ts)))
                    x2 x3 =
-         instantiate (strip arg) n
+         instantiate (compile arg) n
                      (etaExpand (TConstruct x0 x1)
-                                (tcons (strip t) (strips ts)) x2 x3)).
+                                (tcons (compile t) (compile_terms ts)) x2 x3)).
       cbn. induction x2; cbn in *.
       * { destruct x3.
           - rewrite H3. rewrite H5.
@@ -850,7 +899,7 @@ Proof.
 
 
         
-      Eval cbn in (etaExpand (TConstruct x0 x1) (tcons (strip t) (strips ts))).
+      Eval cbn in (etaExpand (TConstruct x0 x1) (tcons (compile t) (compile_terms ts))).
       unfold etaExpand.
       cbn.
       cbn in H1. destruct x2; cbn in *.
@@ -864,31 +913,31 @@ Proof.
 
 
       change
-        (strip
+        (compile
            (L2d.compile.TApp (L2d.compile.TConstruct x0 x1 x2 x3)
                             (L2d.term.instantiate arg n t)
                             (L2d.term.instantiates arg n ts)) =
-         instantiate (strip arg) n
-                     (strip (L2d.compile.TApp
+         instantiate (compile arg) n
+                     (compile (L2d.compile.TApp
                                (L2d.compile.TConstruct x0 x1 x2 x3) t ts))).
       
       change
-        (strip
+        (compile
            (L2d.compile.TApp
               (L2d.compile.TConstruct x0 x1 x2 x3)
               (L2d.term.instantiate arg n t)
               (L2d.term.instantiates arg n ts)) =
          instantiate
-           (strip arg) n
+           (compile arg) n
            (etaExpand (TConstruct x0 x1)
-                      (tcons (instantiate (strip arg) n  (strip t))
-                             (strips ts)) x2 x3)).
+                      (tcons (instantiate (compile arg) n  (compile t))
+                             (compile_terms ts)) x2 x3)).
       change
-        (etaExpand (TConstruct x0 x1) (tcons (strip t) (strips ts)) x2 x3 =
+        (etaExpand (TConstruct x0 x1) (tcons (compile t) (compile_terms ts)) x2 x3 =
          instantiate
-           (strip arg) n
+           (compile arg) n
            (etaExpand (TConstruct x0 x1)
-                      (tcons (strip t) (strips ts)) x2 x3)).
+                      (tcons (compile t) (compile_terms ts)) x2 x3)).
 
       
       rewrite <- etaExpand_instantiate.
@@ -896,60 +945,60 @@ Proof.
       *
       change
         (etaExpand (TConstruct x0 x1)
-                   (tcons (strip (L2d.term.instantiate arg n t))
-                          (strips (L2d.term.instantiates arg n ts))) x2 x3 =
+                   (tcons (compile (L2d.term.instantiate arg n t))
+                          (compile_terms (L2d.term.instantiates arg n ts))) x2 x3 =
          etaExpand (TConstruct x0 x1)
-                   (instantiates (strip arg) n (tcons (strip t) (strips ts)))
+                   (instantiates (compile arg) n (tcons (compile t) (compile_terms ts)))
                    x2 x3).
 
 
     instantiate
-           (strip arg) n
+           (compile arg) n
            (etaExpand (TConstruct x0 x1)
-                      (tcons (strip t) (strips ts)) x2 x3)).
+                      (tcons (compile t) (compile_terms ts)) x2 x3)).
 
       change
         (etaExpand (TConstruct x0 x1)
-                   (tcons (strip (L2d.term.instantiate arg n t))
-                          (strips (L2d.term.instantiates arg n ts))) x2 x3 =
+                   (tcons (compile (L2d.term.instantiate arg n t))
+                          (compile_terms (L2d.term.instantiates arg n ts))) x2 x3 =
          instantiate
-           (strip arg) n
+           (compile arg) n
            (etaExpand (TConstruct x0 x1)
-                      (tcons (strip t) (strips ts)) x2 x3)).
+                      (tcons (compile t) (compile_terms ts)) x2 x3)).
       rewrite H3, H5.
-      Check (etaExpand_TConstruct_instantiate x0 x1 (strip arg) n _ x2 x3).
+      Check (etaExpand_TConstruct_instantiate x0 x1 (compile arg) n _ x2 x3).
 
       destruct x2.
       * cbn. rewrite <- H1.
 
-      unfold strip at 1.
+      unfold compile at 1.
       
       change
-        (strip
+        (compile
            (L2d.compile.TApp (L2d.compile.TConstruct x0 x1 x2 x3)
                             (L2d.term.instantiate arg n t)
                             (L2d.term.instantiates arg n ts)) =
-         instantiate (strip arg) n
-                     (etaExp_cnstr x0 x1 x2 x3 (tcons (strip t) (strips ts)))).
+         instantiate (compile arg) n
+                     (etaExp_cnstr x0 x1 x2 x3 (tcons (compile t) (compile_terms ts)))).
       change
         (etaExp_cnstr x0 x1 x2 x3
-                      (tcons (strip (L2d.term.instantiate arg n t))
-                             (strips (L2d.term.instantiates arg n ts))) =
-         instantiate (strip arg) n
-                     (etaExp_cnstr x0 x1 x2 x3 (tcons (strip t) (strips ts)))).
+                      (tcons (compile (L2d.term.instantiate arg n t))
+                             (compile_terms (L2d.term.instantiates arg n ts))) =
+         instantiate (compile arg) n
+                     (etaExp_cnstr x0 x1 x2 x3 (tcons (compile t) (compile_terms ts)))).
       rewrite H3. rewrite H5.
       change
         (etaExp_cnstr x0 x1 x2 x3
-                      (instantiates (strip arg) n
-                                    (tcons (strip t) (strips ts))) =
-         instantiate (strip arg) n
-                     (etaExp_cnstr x0 x1 x2 x3 (tcons (strip t) (strips ts)))).
-      destruct (etaExp_cnstr_Sanity' x0 x1 x2 x3 (tcons (strip t) (strips ts))).
+                      (instantiates (compile arg) n
+                                    (tcons (compile t) (compile_terms ts))) =
+         instantiate (compile arg) n
+                     (etaExp_cnstr x0 x1 x2 x3 (tcons (compile t) (compile_terms ts)))).
+      destruct (etaExp_cnstr_Sanity' x0 x1 x2 x3 (tcons (compile t) (compile_terms ts))).
       * { rewrite H6.
           destruct (etaExp_cnstr_Sanity'
                       x0 x1 x2 x3 (instantiates
-                                     (strip arg) n (tcons (strip t)
-                                                          (strips ts)))).
+                                     (compile arg) n (tcons (compile t)
+                                                          (compile_terms ts)))).
           - rewrite H7.
          
 
@@ -957,8 +1006,8 @@ Proof.
 Lemma whBetaStep_hom:
   forall bod arg args,
     L2d.term.WFTrm bod 0 ->
-    strip (L2d.term.whBetaStep bod arg args) =
-    whBetaStep (strip bod) (strip arg) (strips args).
+    compile (L2d.term.whBetaStep bod arg args) =
+    whBetaStep (compile bod) (compile arg) (compile_terms args).
 Proof.
   intros bod arg args h.
   unfold L2d.term.whBetaStep, whBetaStep.
@@ -969,27 +1018,27 @@ Proof.
     destruct (L2d.term.isApp_dec (L2d.term.instantiate arg 0 bod)).
     + destruct i as [x0 [x1 [x2 jx]]]. rewrite jx. clear jx.
     change
-      (strip (L2d.compile.TApp
+      (compile (L2d.compile.TApp
                 x0 x1 (L2d.term.tappend x2 (L2d.compile.tcons t args))) =
-       mkApp (strip (L2d.compile.TApp x0 x1 x2))
-             (strips (L2d.compile.tcons t args))).
+       mkApp (compile (L2d.compile.TApp x0 x1 x2))
+             (compile_terms (L2d.compile.tcons t args))).
     destruct (L2d.term.isConstruct_dec x0).
       * { destruct i as [i0 [i1 [i2 [i3 ji]]]]. subst.
         change
           (etaExp_cnstr i0 i1 i2 i3
-                        (tcons (strip x1)
-                               (strips (L2d.term.tappend
+                        (tcons (compile x1)
+                               (compile_terms (L2d.term.tappend
                                           x2 (L2d.compile.tcons t args)))) =
            mkApp (etaExp_cnstr i0 i1 i2 i3
-                        (tcons (strip x1) (strips x2)))
-                 (strips (L2d.compile.tcons t args))).
-        rewrite strips_tappend. rewrite tcons_hom.   
+                        (tcons (compile x1) (compile_terms x2)))
+                 (compile_terms (L2d.compile.tcons t args))).
+        rewrite compile_terms_tappend. rewrite tcons_hom.   
         destruct (etaExp_cnstr_Sanity' i0 i1 i2 i3
-                                        (tcons (strip x1) (strips x2))).
+                                        (tcons (compile x1) (compile_terms x2))).
           - rewrite H. rewrite mkApp_goodFn; try not_isApp.
         destruct (etaExp_cnstr_Sanity' i0 i1 i2 i3
-                                         (tcons (strip x1)
-                                                (compile.tappend (strips x2) (tcons (strip t) (strips args))))).
+                                         (tcons (compile x1)
+                                                (compile.tappend (compile_terms x2) (tcons (compile t) (compile_terms args))))).
         rewrite H0.
 
         rewrite <- (proj1 instantiate_hom); try assumption.
@@ -997,14 +1046,14 @@ Proof.
     + destruct i as [y0 [y1 [y2 [y3 jy]]]]. subst.
       change
         (etaExp_cnstr y0 y1 y2 y3
-                      (tcons (strip x1) (strips (L2d.term.tappend x2 args))) =
+                      (tcons (compile x1) (compile_terms (L2d.term.tappend x2 args))) =
          mkApp (etaExp_cnstr y0 y1 y2 y3
-                             (tcons (strip x1) (strips x2)))
-               (strips args)).
+                             (tcons (compile x1) (compile_terms x2)))
+               (compile_terms args)).
       destruct (etaExp_cnstr_Sanity'
                   y0 y1 y2 y3
-                  (tcons (strip x1) (strips (L2d.term.tappend x2 args)))),
-      (etaExp_cnstr_Sanity'  y0 y1 y2 y3 (tcons (strip x1) (strips x2)));
+                  (tcons (compile x1) (compile_terms (L2d.term.tappend x2 args)))),
+      (etaExp_cnstr_Sanity'  y0 y1 y2 y3 (tcons (compile x1) (compile_terms x2)));
         rewrite H; rewrite H0.
       * { cbn. destruct args. cbn.
           - apply f_equal3; try reflexivity.
@@ -1015,8 +1064,8 @@ Proof.
 (****
 Goal
   forall i n npars nargs arg args,
-  etaExp_cnstr i n npars nargs (tcons (strip arg) (strips args)) =
-  TApp (etaExp_cnstr i n npars nargs tnil) (strip arg) (strips args).
+  etaExp_cnstr i n npars nargs (tcons (compile arg) (compile_terms args)) =
+  TApp (etaExp_cnstr i n npars nargs tnil) (compile arg) (compile_terms args).
 Proof.
   intros. induction args.
   - cbn. induction npars.
@@ -1026,12 +1075,12 @@ Proof.
 (****
 Lemma mkApp_hom:
 forall fn args, ~ L2d.term.isApp fn ->
-  strip (L2d.term.mkApp fn args) = mkApp (strip fn) (strips args).
+  compile (L2d.term.mkApp fn args) = mkApp (compile fn) (compile_terms args).
 Proof.
   intros. destruct args.
   - rewrite L2d.term.mkApp_tnil_ident. rewrite mkApp_tnil_ident. reflexivity.
   - rewrite L2d.term.mkApp_goodFn; try assumption. 
-    assert (j: ~ isApp (strip fn)).
+    assert (j: ~ isApp (compile fn)).
     { intros h. elim H. apply isApp_hom. assumption. }
 
   
@@ -1042,17 +1091,17 @@ Admitted.
   intros. destruct args.
   - rewrite L2d.term.mkApp_tnil_ident. rewrite mkApp_tnil_ident. reflexivity.
   - rewrite L2d.term.mkApp_goodFn; try assumption. rewrite tcons_hom.
-    assert (j: ~ isApp (strip fn)).
+    assert (j: ~ isApp (compile fn)).
     { intros h. elim H. apply isApp_hom. assumption. }
     rewrite mkApp_goodFn; try assumption. destruct fn; try (cbn; reflexivity).
     change
-      (etaExp_cnstr i n n0 n1 (tcons (strip t) (strips args)) =
-       TApp (strip (L2d.compile.TConstruct i n n0 n1)) (strip t) (strips args)).
+      (etaExp_cnstr i n n0 n1 (tcons (compile t) (compile_terms args)) =
+       TApp (compile (L2d.compile.TConstruct i n n0 n1)) (compile t) (compile_terms args)).
     change
-      (etaExp_cnstr i n n0 n1 (tcons (strip t) (strips args)) =
-       TApp (etaExp_cnstr i n n0 n1 tnil) (strip t) (strips args)).
+      (etaExp_cnstr i n n0 n1 (tcons (compile t) (compile_terms args)) =
+       TApp (etaExp_cnstr i n n0 n1 tnil) (compile t) (compile_terms args)).
            
-    unfold strip in j.
+    unfold compile in j.
     
   destruct args; try (reflexivity).
   - rewrite L2d.term.mkApp_tnil_ident. rewrite mkApp_tnil_ident.
@@ -1063,7 +1112,7 @@ Admitted.
       destruct (L2d.term.isConstruct_dec fn).
       * { destruct H as [x0 [x1 [x2 [x3 jx]]]]. subst. cbn.
           destruct (etaExp_cnstr_Sanity'
-                      x0 x1 x2 x3 (tcons (strip t) (strips args))).
+                      x0 x1 x2 x3 (tcons (compile t) (compile_terms args))).
           - destruct H as [y0 [y1 [y2 jy]]]. rewrite jy.
             destruct (etaExp_cnstr_Sanity' x0 x1 x2 x3 tnil).
             + destruct H as [z0 [z1 [z2 jz]]]. rewrite jz. cbn. rewrite <- jy.
@@ -1073,7 +1122,7 @@ Admitted.
               destruct (etaExp_cnstr_Sanity' x0 x1 x2 x3 tnil).
           
           assert (j:= etaExp_cnstr_Sanity
-                        x0 x1 x2 x3 (tcons (strip t) (strips args))).
+                        x0 x1 x2 x3 (tcons (compile t) (compile_terms args))).
           rewrite TApp_hom. admit. ; try assumption.
 
     case_eq fn; intros; try reflexivity.
@@ -1094,10 +1143,10 @@ Proof.
 Qed.
 ***)
 
-Lemma isApp_strip:
+Lemma isApp_compile:
   forall fn,
     ~ L2d.term.isConstruct fn ->
-    forall arg args, strip (L2d.compile.TApp fn arg args) = TApp (strip fn) (strip arg) (strips args).
+    forall arg args, compile (L2d.compile.TApp fn arg args) = TApp (compile fn) (compile arg) (compile_terms args).
 Proof.
   destruct fn; cbn; intros; auto. elim H. auto.
 Qed.
@@ -1141,19 +1190,19 @@ Proof.
 (****
 Goal
   forall arg n t s,
-    CanonicalP strip t (strip s) = Some (i, m, us, np, na) ->
-    instantiate (strip arg) n 
-      CanonicalP strip (L2d.term.instantiate arg n t)
-           (strip (L2d.term.instantiate arg n s)) =
-      instantiate (strip arg) n (CanonicalP strip t (strip s)).         
+    CanonicalP compile t (compile s) = Some (i, m, us, np, na) ->
+    instantiate (compile arg) n 
+      CanonicalP compile (L2d.term.instantiate arg n t)
+           (compile (L2d.term.instantiate arg n s)) =
+      instantiate (compile arg) n (CanonicalP compile t (compile s)).         
 ***************)
   
 (****
 Goal
   forall arg n t s,
-    CanonicalP strip t (strip s) = None ->
-      CanonicalP strip (L2d.term.instantiate arg n t)
-           (strip (L2d.term.instantiate arg n s)) = None.
+    CanonicalP compile t (compile s) = None ->
+      CanonicalP compile (L2d.term.instantiate arg n t)
+           (compile (L2d.term.instantiate arg n s)) = None.
 Proof.
   induction t; intros.
   - cbn. destruct (nat_compare n n0).
@@ -1165,17 +1214,17 @@ Proof.
 (***  essential *****
 Lemma instantiate_hom:
   (forall bod arg n,
-     strip (L2d.term.instantiate arg n bod) =
-     instantiate (strip arg) n (strip bod)) /\
+     compile (L2d.term.instantiate arg n bod) =
+     instantiate (compile arg) n (compile bod)) /\
   (forall bods arg n,
-     strips (L2d.term.instantiates arg n bods) =
-     instantiates (strip arg) n (strips bods)) /\
+     compile_terms (L2d.term.instantiates arg n bods) =
+     instantiates (compile arg) n (compile_terms bods)) /\
   (forall bods arg n,
-     stripBs (L2d.term.instantiateBrs arg n bods) =
-     instantiateBrs (strip arg) n (stripBs bods)) /\
+     compileBs (L2d.term.instantiateBrs arg n bods) =
+     instantiateBrs (compile arg) n (compileBs bods)) /\
   (forall ds arg n,
-          stripDs (L2d.term.instantiateDefs arg n ds) =
-     instantiateDefs (strip arg) n (stripDs ds)).
+          compile_defs (L2d.term.instantiateDefs arg n ds) =
+     instantiateDefs (compile arg) n (compile_defs ds)).
 Proof.
   apply L2d.compile.TrmTrmsBrsDefs_ind; intros; try (cbn; reflexivity);
   try (cbn; rewrite H; reflexivity).
@@ -1186,50 +1235,50 @@ Proof.
     + rewrite (proj1 (nat_compare_gt n0 n)); trivial.
   - cbn. rewrite H. rewrite H0. reflexivity.
   - change
-      (strip (L2d.compile.TApp (L2d.term.instantiate arg n t)
+      (compile (L2d.compile.TApp (L2d.term.instantiate arg n t)
                                (L2d.term.instantiate arg n t0)) =
-       instantiate (strip arg) n (strip (L2d.compile.TApp t t0))).
+       instantiate (compile arg) n (compile (L2d.compile.TApp t t0))).
     rewrite TApp_hom. rewrite TApp_hom.
     rewrite H0. rewrite H.
 
-    destruct (CanonicalP strip (L2d.term.instantiate arg n t)
-                         (strip (L2d.term.instantiate arg n t0))).
+    destruct (CanonicalP compile (L2d.term.instantiate arg n t)
+                         (compile (L2d.term.instantiate arg n t0))).
     + repeat (destruct p). 
-      destruct (CanonicalP strip t (strip t0)).
+      destruct (CanonicalP compile t (compile t0)).
       * repeat (destruct p).
 
       
     - admit. (***  cbn. rewrite H. rewrite H0. reflexivity. ***)
   - change
-      (strip (L2d.term.instantiate arg n2 (L2d.compile.TConstruct i n n0 n1)) =
-       instantiate (strip arg) n2 (strip (L2d.compile.TConstruct i n n0 n1))).
-    unfold strip at 3.
+      (compile (L2d.term.instantiate arg n2 (L2d.compile.TConstruct i n n0 n1)) =
+       instantiate (compile arg) n2 (compile (L2d.compile.TConstruct i n n0 n1))).
+    unfold compile at 3.
     cbn. destruct n0.
     +
     
-      (strip (term.instantiate arg n0 (L2d.compile.TConstruct i n t)) =
-       TConstruct i n (instantiates (strip arg) n0 (strips t))).
+      (compile (term.instantiate arg n0 (L2d.compile.TConstruct i n t)) =
+       TConstruct i n (instantiates (compile arg) n0 (compile_terms t))).
     rewrite <- H; trivial.
   - change
-     (TCase i (strip (L2d.term.instantiate arg n t))
-            (stripBs (L2d.compile.instantiateBrs arg n b)) =
-      TCase i (instantiate (strip arg) n (strip t))
-            (instantiateBrs (strip arg) n (stripBs b))).
+     (TCase i (compile (L2d.term.instantiate arg n t))
+            (compileBs (L2d.compile.instantiateBrs arg n b)) =
+      TCase i (instantiate (compile arg) n (compile t))
+            (instantiateBrs (compile arg) n (compileBs b))).
     rewrite H; trivial. rewrite H0; trivial.
   - change
       (TFix
-         (stripDs (L2d.term.instantiateDefs
+         (compile_defs (L2d.term.instantiateDefs
                      arg (n0 + (L2d.compile.dlength d)) d)) n =
        TFix (instantiateDefs
-               (strip arg) (n0 + (dlength (stripDs d))) (stripDs d)) n).
-    rewrite H. rewrite stripDs_pres_dlength. reflexivity.
-  - rewrite L2d.stripEvalCommute.instantiates_tcons_commute.
+               (compile arg) (n0 + (dlength (compile_defs d))) (compile_defs d)) n).
+    rewrite H. rewrite compile_defs_pres_dlength. reflexivity.
+  - rewrite L2d.compileEvalCommute.instantiates_tcons_commute.
     rewrite tcons_hom. rewrite tcons_hom. rewrite instantiates_tcons.
     rewrite <- H; trivial. rewrite H0; trivial.
-  - rewrite L2d.stripEvalCommute.instantiates_bcons_commute.
+  - rewrite L2d.compileEvalCommute.instantiates_bcons_commute.
     rewrite bcons_hom. rewrite bcons_hom. rewrite instantiateBs_bcons.
     rewrite <- H; trivial. rewrite H0; trivial.
-  - rewrite L2d.stripEvalCommute.instantiates_dcons_commute.
+  - rewrite L2d.compileEvalCommute.instantiates_dcons_commute.
     rewrite dcons_hom. rewrite dcons_hom. rewrite instantiateDs_dcons.
     rewrite <- H; trivial. rewrite H0; trivial.
 Qed.
@@ -1243,16 +1292,17 @@ Qed.
 
 Lemma TLambda_hom:
   forall nm bod,
-    strip (L1g.compile.TLambda nm bod) = TLambda nm (strip bod).
-reflexivity.
+    compile (tLambda nm bod) = TLambda nm (compile bod).
+Proof.
+  intros. now simp_compile.
 Qed.
 
-Lemma whBetaStep_hom:
+(* Lemma whBetaStep_hom:
   forall bod arg,
-    strip (L1g.term.whBetaStep bod arg) =
-    whBetaStep (strip bod) (strip arg).
+    compile (L1g.term.whBetaStep bod arg) =
+    whBetaStep (compile bod) (compile arg).
 Proof.
-Admitted.
+Admitted. *)
 (*************
   intros. unfold L2d.term.whBetaStep, whBetaStep.
   Check (proj1 instantiate_hom).
@@ -1260,118 +1310,804 @@ Admitted.
 Qed.
  **************)
 
-(************* MAIN *************
-Lemma WcbvEval_hom:
-  forall p,
-    (forall t t', L2d.wcbvEval.WcbvEval p t t' ->
-                  WcbvEval (stripEnv p) (strip t) (strip t')) /\
-    (forall ts ts', L2d.wcbvEval.WcbvEvals p ts ts' ->
-                    WcbvEvals (stripEnv p) (strips ts) (strips ts')).
+End OnGlobalEnv.
+
+(************* MAIN *************)
+
+Lemma well_formed_pres (efl := all_env_flags) Σ : wf_glob Σ -> Qpreserves (wellformed Σ) Σ.
+Proof. Admitted.
+From Equations Require Import Equations.
+
+Lemma compile_mkApps Σ fn args :
+  negb (EAst.isApp fn) ->
+  compile Σ (mkApps fn args) =
+    match construct_viewc fn with
+    | view_construct kn c => 
+      match lookup_constructor_pars_args Σ kn c with
+      | Some (npars, nargs) => 
+        let args := map (compile Σ) args in
+        let '(args, rest) := MCList.chop nargs args in
+        TmkApps (TConstruct kn c (list_terms args)) (list_terms rest)
+      | None =>
+        let args := compile_terms Σ args in
+        TConstruct kn c args
+      end
+    | view_other fn nconstr =>
+        TmkApps (compile Σ fn) (compile_terms Σ args)
+    end.
 Proof.
-  intros p.
-  apply L2d.wcbvEval.WcbvEvalEvals_ind; intros; try reflexivity;
-    try (solve[constructor; trivial]).
-  - unfold strip. destruct np.
-    + unfold etaExpand. unfold etaExpand_args_Construct. destruct na.
-      * econstructor. econstructor.
-      *{ destruct (isLambda_etaExpand_args_Lam_Lam
-                     na tnil (TConstruct i r) (tunit (TRel 0))).
-         - dstrctn H. rewrite j. constructor.
-         - dstrctn H. rewrite j. constructor. }
-    + unfold etaExpand. destruct (nLambda_isLambda np (TConstruct i r)).
-      rewrite H.
-      destruct (isLambda_etaExpand_args_Lam_Lam na tnil x tnil). 
-      * dstrctn H0. rewrite j. constructor.
-      * dstrctn H0. rewrite j. constructor.
-  - cbn. econstructor; try eassumption.
-    + apply lookupDfn_hom. eassumption.
-  - rewrite TApp_hom. cbn. destruct (CanonicalP strip fn (strip a1)).
-    + admit.  (**** eta expand  ***
-destruct p0 as [[[[y0 y1] y2] y3] y4].
-      destruct (isLambda_etaExpand y4 y2 y0 y1 y3) as [h|[h|h]].
-      * dstrctn h. rewrite j. eapply wAppLam.
-          unfold lifts. unfold compile.tappend. induction na.
-         - cbn. econstructor. econstructor. econstructor. econstructor.
-               *****************)
-    + rewrite TLambda_hom in H. eapply wAppLam; try eassumption.
-Check whBetaStep_hom.
-
-unfold etaExpand_args_Lam.
-  - cbn. destruct np; cbn.
-    + destruct na; cbn. econstructor.
-
-  - cbn. destruct np; cbn.
-    + destruct na; cbn.
-      * constructor. constructor.
-      * assert (j: na >= tlength tnil). cbn. omega.
-        destruct (@na_isLambda_etaExpand_args
-                 na tnil j (fun b => TConstruct i r b)
-                 (tunit (TRel 0))) as [x0 [x1 jx]].
-        rewrite jx. constructor.
-    + assert (j: na >= tlength tnil). cbn. omega.
-      destruct (@na_isLambda_etaExpand_args
-                  na tnil j (fun b => TConstruct i r b) tnil)
-        as [x0 [x1 jx]]. rewrite jx. constructor.
-  - cbn. econstructor; try eassumption. apply lookupDfn_hom. assumption.
-  - destruct (L2d.term.isConstruct_dec fn).
-    + destruct i as [x0 [x1 [x2 [x3 jx]]]]. subst.
-      inversion_Clear w.
-    + simpl. destruct fn; cbn; try inversion_Clear w.
-
-      cbn in H. econstructor; try eassumption.
-
-      
-    + rewrite (isApp_strip n a1 args). eapply wAppLam. eassumption. eapply H0.
-      change
-        (WcbvEval (stripEnv p) (strip (L2d.term.whBetaStep bod a1' args)) (strip s)) in H1.
-
-
-      unfold strip at 1 in H1. eapply H1.
-      cbn.
-      change
-        (WcbvEval (stripEnv p) (strip (L2d.compile.TApp fn a1 args)) (strip s)).
-      change
-        (WcbvEval (stripEnv p) (strip (L2d.compile.TApp fn a1 args)) (strip s)).
-
-  - cbn. eapply wAppLam.
-    + apply H. 
-    + apply H0. 
-    + rewrite whBetaStep_hom in H1. assumption.
-  - cbn. eapply wLetIn.
-    + apply H. 
-    + rewrite <- (proj1 instantiate_hom). assumption.
-  - cbn. eapply wAppFix.
-    + eapply H.
-    + rewrite <- dnthBody_hom. rewrite e. reflexivity.
-    + rewrite <- pre_whFixStep_hom in H0. eapply H0.
-  - destruct (WcbvEvals_tcons_tcons H0) as [a' [args' j]]. rewrite j in H0.
-    cbn. rewrite mkApp_hom. eapply wAppCong. try eassumption.
-    + intros h. elim n. apply isLambda_hom. assumption.
-    + intros h. elim n0. apply isFix_hom. assumption.
-    + rewrite j. cbn in H0. assumption.
-  - refine (wCase _ _ _ _ _ _ _); try eassumption.
-    * rewrite <- canonicalP_hom. rewrite e. reflexivity.
-    * rewrite <- tskipn_hom. rewrite e0. reflexivity.
-    * rewrite <- whCaseStep_hom. rewrite e1. reflexivity.
-  - refine (wCaseCong _ _ _ _); try eassumption.
-    + rewrite <- canonicalP_hom. rewrite e. reflexivity.
+  intros napp; simp compile.
+  destruct (construct_viewc fn) eqn:vc.
+  - destruct lookup_constructor_pars_args as [[]|] eqn:heq.
+    destruct args eqn:hargs. cbn.
+    * destruct n1 => //.
+    * set (v := TermSpineView.view _).
+      destruct (TermSpineView.view_mkApps v) as [hf [vn eq]] => //.
+      rewrite eq /=. rewrite heq /=. now simp_compile.
+    * destruct args eqn:hargs => //.
+      set (v := TermSpineView.view _).
+      destruct (TermSpineView.view_mkApps v) as [hf [vn eq]] => //.
+      rewrite eq /=. rewrite heq /=. now simp_compile.
+  - destruct args eqn:hargs => //.
+    simp compile. now cbn.  
+    set (v := TermSpineView.view _).
+    destruct (TermSpineView.view_mkApps v) as [hf [vn eq]] => //.
+    rewrite eq /= vc /=. now simp_compile.
 Qed.
-*****)
+
+From Coq Require Import ssrbool.
+
+Lemma wellformed_lookup_inductive_pars Σ kn mdecl :
+  wf_glob Σ ->
+  lookup_minductive Σ kn = Some mdecl -> mdecl.(ind_npars) = 0.
+Proof.
+  induction 1; cbn => //.
+  case: eqb_spec => [|].
+  - intros ->. destruct d => //. intros [= <-].
+    cbn in H0. now eapply eqb_eq in H0.
+  - intros _. eapply IHwf_glob.
+Qed.
+
+Lemma wellformed_lookup_constructor_pars {Σ kn c mdecl idecl cdecl} :
+  wf_glob Σ ->
+  lookup_constructor Σ kn c = Some (mdecl, idecl, cdecl) -> mdecl.(ind_npars) = 0.
+Proof.
+  intros wf. cbn -[lookup_minductive].
+  destruct lookup_minductive eqn:hl => //.
+  do 2 destruct nth_error => //.
+  eapply wellformed_lookup_inductive_pars in hl => //. congruence.
+Qed.
+
+Lemma lookup_constructor_pars_args_spec {Σ ind n mdecl idecl cdecl} :
+  wf_glob Σ ->
+  lookup_constructor Σ ind n = Some (mdecl, idecl, cdecl) ->
+  lookup_constructor_pars_args Σ ind n = Some (mdecl.(ind_npars), cdecl.2).
+Proof.
+  cbn -[lookup_constructor] => wfΣ.
+  destruct lookup_constructor as [[[mdecl' idecl'] [pars args]]|] eqn:hl => //.
+  intros [= -> -> <-]. cbn. f_equal.
+Qed.
+
+Lemma wellformed_lookup_constructor_pars_args {Σ ind n} :
+  wf_glob Σ ->
+  wellformed Σ 0 (EAst.tConstruct ind n) ->
+  ∑ args, lookup_constructor_pars_args Σ ind n = Some (0, args).
+Proof.
+  intros wfΣ wf. cbn -[lookup_constructor] in wf.
+  destruct lookup_constructor as [[[mdecl idecl] cdecl]|] eqn:hl => //.
+  exists cdecl.2.
+  pose proof (wellformed_lookup_constructor_pars wfΣ hl).
+  eapply lookup_constructor_pars_args_spec in hl => //. congruence.
+Qed.
+
+Lemma constructor_isprop_pars_decl_params {Σ ind c b pars cdecl} :
+  wf_glob Σ ->
+  constructor_isprop_pars_decl Σ ind c = Some (b, pars, cdecl) -> pars = 0.
+Proof.
+  intros hwf.
+  rewrite /constructor_isprop_pars_decl /lookup_constructor /lookup_inductive.
+  destruct lookup_minductive as [mdecl|] eqn:hl => /= //.
+  do 2 destruct nth_error => //.
+  eapply wellformed_lookup_inductive_pars in hl => //. congruence.
+Qed.
+
+Lemma compile_mkApps_wf (P : Term -> Prop) Σ k fn args :
+  wf_glob Σ -> 
+  ~~ EAst.isApp fn ->
+  wellformed Σ k (mkApps fn args) ->
+  (match construct_viewc fn with
+  | view_construct kn c => 
+    match lookup_constructor_pars_args Σ kn c with
+    | Some (0, nargs) => 
+      let cargs := map (compile Σ) args in
+      let '(cargs, rest) := MCList.chop nargs cargs in
+      P (TConstruct kn c (list_terms cargs))
+    | _ => True
+    end
+  | view_other fn nconstr =>
+      P (TmkApps (compile Σ fn) (list_terms (map (compile Σ) args)))
+  end) ->
+  P (compile Σ (mkApps fn args)).
+Proof.
+  intros wfΣ napp.
+  rewrite wellformed_mkApps // => /andP[] wffn wfargs.
+  destruct construct_viewc eqn:vc.
+  + rewrite compile_mkApps // vc.
+    destruct (wellformed_lookup_constructor_pars_args wfΣ wffn).
+    rewrite e. cbn.
+    destruct chop eqn:eqch => //. 
+  + intros ht. rewrite compile_mkApps // vc //.
+Qed.
+
+Lemma compile_decompose Σ f :
+  compile Σ f =
+  let (fn, args) := decompose_app f in
+    match construct_viewc fn with
+    | view_construct kn c => 
+      match lookup_constructor_pars_args Σ kn c with
+      | Some (npars, nargs) => 
+        let args := map (compile Σ) args in
+        let '(args, rest) := MCList.chop nargs args in
+        TConstruct kn c (list_terms args)
+      | None =>
+        let args := compile_terms Σ args in
+        TConstruct kn c args
+      end
+    | view_other fn nconstr =>
+        TmkApps (compile Σ fn) (compile_terms Σ args)
+    end.
+Proof.
+  destruct (decompose_app f) eqn:da.
+  rewrite (decompose_app_inv da). apply compile_mkApps.
+  now eapply decompose_app_notApp.
+Qed.
+
+
+Inductive Forall2_terms (P : Term -> Term -> Prop) : Terms -> Terms -> Prop :=
+  | Forall2_nil_terms : Forall2_terms P tnil tnil
+  | Forall2_cons_terms t t' l l' : P t t' -> Forall2_terms P l l' -> Forall2_terms P (tcons t l) (tcons t' l').
+
+Section Reverse_Induction.
+  Lemma trev_list_ind :
+    forall P:Terms -> Type,
+      P tnil ->
+        (forall (a:Term) (l:Terms), P (treverse l) -> P (treverse (tcons a l))) ->
+        forall l, P (treverse l).
+  Proof.
+    induction l; auto.
+  Qed.
+
+  Theorem trev_ind :
+    forall P:Terms -> Type,
+      P tnil ->
+      (forall x l, P l -> P (tappend l (tcons x tnil))) -> forall l, P l.
+  Proof.
+    intros.
+    generalize (treverse_involutive l).
+    intros E; rewrite <- E.
+    apply (trev_list_ind P).
+    auto.
+
+    simpl.
+    intros.
+    apply (X0 a (treverse l0)).
+    auto.
+  Qed.
+
+End Reverse_Induction.
+
+Derive Signature for WcbvEval.
+Derive NoConfusion for Term Terms.
+
+Lemma TmkApps_tappend f args args' : TmkApps f (tappend args args') = TmkApps (TmkApps f args) args'.
+Proof.
+  induction args in args' |- * using trev_ind.
+  - cbn => //. 
+  - cbn.
+    rewrite IHargs /=.
+    rewrite -tappend_assoc. rewrite IHargs //=. 
+Qed.
+
+Lemma eval_mkAppsConstruct_inv' :
+  forall p t x, WcbvEval p t x -> 
+  forall f args, t = TmkApps f args -> 
+  forall i r args', f = TConstruct i r args' -> 
+  args = tnil /\ exists argsv, WcbvEvals p args' argsv /\ x = TConstruct i r argsv.
+Proof.
+  intros p t x ev f args.
+  induction args in f, t, x, ev |- *using trev_ind. cbn.
+  - intros -> i r args' ->.
+    split => //. 
+    depind ev; try discriminate. exists args'. split => //.
+  - cbn.
+    intros ht i r args' ->.
+    rewrite ht in ev. rewrite !TmkApps_tappend /= in ev.
+    cbn in ev. depelim ev.
+    specialize (IHargs _ _ ev1 _ eq_refl _ _ _ eq_refl) as [? [? []]]. discriminate.
+    specialize (IHargs _ _ ev1 _ eq_refl _ _ _ eq_refl) as [? [? []]]. discriminate.
+    specialize (IHargs _ _ ev1 _ eq_refl _ _ _ eq_refl) as [? [? []]]. discriminate.
+    specialize (IHargs _ _ ev1 _ eq_refl _ _ _ eq_refl) as [? [? []]]. subst fn'.
+    destruct H as [? [? []]]. elim H3. now eauto.
+Qed.
+
+Lemma eval_TmkApps_Construct_inv :
+  forall p i r args' args x, WcbvEval p (TmkApps (TConstruct i r args') args) x -> 
+  args = tnil /\ exists argsv, WcbvEvals p args' argsv /\ x = TConstruct i r argsv.
+Proof.
+  intros. eapply eval_mkAppsConstruct_inv'; trea.
+Qed.
+
+Lemma TApp_TmkApps f l t : TApp (TmkApps f l) t = TmkApps f (tappend l (tunit t)).
+Proof.
+  rewrite TmkApps_tappend //.
+Qed.
+
+Lemma eval_to_mkApps_Construct_inv_gen :
+  forall p t x, WcbvEval p t x -> 
+  forall f args, x = TmkApps f args ->
+  args <> tnil -> ~ isConstruct f. 
+Proof.
+  intros p t x ev f args -> hargs.
+  destruct args using trev_ind. congruence. cbn in ev.
+  rewrite -TApp_TmkApps in ev. clear IHargs. clear hargs.
+  depind ev; auto.
+  destruct H as [? [? []]].
+  destruct args using trev_ind. cbn in *. apply H1. 
+  clear IHargs.
+  intros [ind [n [args' eq]]].
+  subst f. eapply IHev1. rewrite TApp_TmkApps. reflexivity.
+  now do 3 eexists.
+Qed.
+
+Definition eq_nil_dec l : l = tnil \/ l <> tnil.
+Proof.
+  destruct l; auto. right; congruence.
+Qed.
+
+Lemma eval_to_mkApps_Construct_inv p t ind c args args' :
+  WcbvEval p t (TmkApps (TConstruct ind c args) args') -> args' = tnil.
+Proof.
+  move/eval_to_mkApps_Construct_inv_gen.
+  intros Hf.
+  specialize (Hf (TConstruct ind c args) _ eq_refl).
+  destruct (eq_nil_dec args') => //.
+  specialize (Hf H). elim Hf. now do 3 eexists.
+Qed.
+
+
+(* Lemma tappend_compile_terms : tappend (compile_terms Σ l) (compile_terms Σ l') = compile_terms (l ++ l'). *)
+
+Lemma compile_tApp Σ t a (P : Term -> Prop) k :
+  wf_glob Σ -> 
+  wellformed Σ k (tApp t a) ->
+  (let (fn, args) := decompose_app (tApp t a) in
+  match construct_viewc fn with
+  | view_construct kn c => 
+    match lookup_constructor_pars_args Σ kn c with
+    | Some (0, nargs) => 
+      let cargs := map (compile Σ) args in
+      let '(cargs, rest) := MCList.chop nargs cargs in
+      (args <> [] /\ t = mkApps (tConstruct kn c) (remove_last args) /\ a = last args a) ->
+      P (TConstruct kn c (list_terms cargs))
+    | _ => True
+    end
+  | view_other fn nconstr =>
+      P (TApp (compile Σ t) (compile Σ a))
+  end) ->
+  P (compile Σ (tApp t a)).
+Proof.
+  intros wfΣ wf.
+  rewrite (compile_decompose _ (tApp t a)).
+  destruct decompose_app eqn:da.
+  pose proof (decompose_app_notApp _ _ _ da).
+  pose proof (EInduction.decompose_app_app _ _ _ _ da).
+  destruct construct_viewc eqn:vc.
+  + eapply EEtaExpandedFix.decompose_app_tApp_split in da as [Ha Ht].
+    cbn in wf.
+    move: wf => /andP[]. rewrite Ha wellformed_mkApps // => /andP[] wfc wfl wft.
+    destruct (wellformed_lookup_constructor_pars_args wfΣ wfc).
+    rewrite e. cbn.
+    destruct chop eqn:eqch => //. 
+    intros. apply H1. intuition auto.
+  + pose proof (decompose_app_notApp _ _ _ da).
+    pose proof (EInduction.decompose_app_app _ _ _ _ da).
+    eapply EEtaExpandedFix.decompose_app_tApp_split in da as [Ha Ht].
+    rewrite Ha Ht.
+    rewrite compile_mkApps // vc.
+    rewrite TApp_TmkApps.
+    rewrite -(tappend_hom _ (remove_last l) [_]).
+    rewrite -remove_last_last //. 
+Qed.
+
+Derive Signature for crctTerms.
+
+Lemma crctTerm_tmkApps Σ n f args : 
+  crctTerm Σ n f ->
+  crctTerms Σ n args ->
+  crctTerm Σ n (TmkApps f args).
+Proof.
+  induction args in f |- *. cbn; auto.
+  intros hf hargs. depelim hargs.
+  cbn. eapply IHargs => //. constructor => //.
+Qed. 
+
+From MetaCoq.SafeChecker Require PCUICTypeChecker.
+
+Ltac simp_eta_in := match goal with [ H : is_true (isEtaExp _ _) |- _ ] => simp_eta in H end.
+
+Lemma compile_isLambda Σ t : EAst.isLambda t -> isLambda (compile Σ t).
+Proof. destruct t => //. now simp_compile. Qed.
+
+Lemma wellformed_eta_crct {Σ} t :
+  isEtaExp_env Σ -> wf_glob Σ ->
+  crctEnv (compile_ctx Σ) ->
+  forall k, wellformed Σ k t ->
+  isEtaExp Σ t -> 
+  crctTerm (compile_ctx Σ) k (compile Σ t).
+Proof.
+  intros etaΣ wfΣ crctΣ.
+  revert t. apply: EInduction.MkAppsInd.rec; cbn [wellformed]; intros; try simp_eta_in; simp_eta; simp_compile.
+  all:intros; simp_compile; rtoProp; intuition auto; try cbn in *; try constructor; eauto.
+  - now eapply Nat.ltb_lt.
+  - simp_compile. 
+    move: H2; rewrite wellformed_mkApps // => /andP[] wfc wfu.
+    move/isEtaExp_mkApps: H3. 
+    rewrite decompose_app_mkApps //. destruct t => //.
+    eapply compile_mkApps_wf => //. rewrite wellformed_mkApps //. now erewrite wfc, wfu.
+    destruct construct_viewc.
+    * destruct lookup_constructor_pars_args as [[[] nargs]|] eqn:heq => //.
+      cbn. rewrite PCUICTypeChecker.chop_firstn_skipn.
+      move/andP=> [] etaind etau.
+      constructor.
+      unfold isEtaExp_app in etaind. rewrite heq in etaind.
+      eapply Nat.leb_le in etaind. todo "crctInd".
+      todo "all".
+    * move/andP=> [] etat etau.
+      eapply crctTerm_tmkApps; eauto.
+      todo "all".
+  - econstructor; tea. todo "const".
+  - todo "eta".
+  - todo "case".
+  - destruct s as [[] ?]. simp_compile.
+    destruct (lookup_record_projs) eqn:hprojs.
+    all:todo "projs".
+  - cbn. rewrite -dlength_hom. 
+    rewrite Nat.add_comm. eapply forallb_All in H1. eapply forallb_All in H0.
+    eapply All_mix in X; tea. clear H0; eapply All_mix in X. 2:exact H1. clear H1.
+    move: X. generalize (#|m| + k).
+    induction 1; try solve [constructor; cbn; auto].
+    intuition auto.
+    move/andP: a0 => [] isl etab.
+    constructor; eauto.
+    now eapply compile_isLambda.
+  - cbn. rewrite -dlength_hom.
+    todo "missing condition in wellformed idx < #|mfix|".
+Admitted.
+
+Lemma wellformed_eta_crctEnv {Σ} :
+  isEtaExp_env Σ -> wf_glob Σ ->
+  crctEnv (compile_ctx Σ).
+Proof.
+  induction Σ; cbn.
+  - constructor.
+  - move/andP=> [] etad etae wf. depelim wf.
+    destruct d.
+    * cbn. destruct c as [[b|]]; econstructor; eauto.
+      todo "fresh". 
+      eapply wellformed_eta_crct => //. eauto.
+      todo "fresh".
+    * constructor; eauto.
+      todo "fresh".
+Qed.
+    
+Lemma isLambda_substl s t : EAst.isLambda t -> EAst.isLambda (ECSubst.substl s t).
+Proof. induction s in t |- * => //.
+  intros isl. cbn. 
+  eapply IHs. destruct t => //.
+Qed.
+
+Local Lemma decompose_app_app t u f l : decompose_app (tApp t u) = (f, l) -> l <> [].
+Proof.
+  intros da.
+  pose proof (decompose_app_inv da).
+  intros ->. cbn in H. subst f.
+  now move: (decompose_app_notApp _ _ _ da).
+Defined.
+
+Lemma list_terms_app l l' : list_terms (l ++ l') = tappend (list_terms l) (list_terms l').
+Proof.
+  induction l in l' |- *.
+  - cbn; auto.
+  - cbn. now f_equal.
+Qed.
+
+Lemma compile_terms_tappend Σ l l' : 
+  compile_terms Σ (l ++ l') = tappend (compile_terms Σ l) (compile_terms Σ l').
+Proof.
+  rewrite /compile_terms map_app list_terms_app //.
+Qed.
+
+Lemma isLambda_compile Σ f : 
+  ~~ EAst.isLambda f -> ~ isLambda (compile Σ f).
+Proof.
+  intros nf. move=> [] na [] bod.
+  destruct f; simp_compile => /= //.
+  2:{ destruct p as [[] ?]; simp_compile => /= //.
+      destruct lookup_record_projs => /= //. }
+  rewrite compile_decompose.
+  destruct decompose_app eqn:da.
+  destruct construct_viewc.
+  destruct lookup_constructor_pars_args as [[[] args]|] => //; cbn; destruct chop eqn:eqc; 
+  destruct (list_terms l1) using trev_ind => //; rewrite -TApp_TmkApps //.
+  eapply decompose_app_app in da. destruct l using rev_ind => //.
+  rewrite compile_terms_tappend // -TApp_TmkApps //.
+Qed.
+
+Lemma isBox_compile Σ f : 
+  ~~ EAstUtils.isBox f -> compile Σ f <> TProof.
+Proof.
+  intros nf.
+  destruct f; simp_compile => /= //.
+  2:{ destruct p as [[] ?]; simp_compile => /= //.
+      destruct lookup_record_projs => /= //. }
+  rewrite compile_decompose.
+  destruct decompose_app eqn:da.
+  destruct construct_viewc.
+  destruct lookup_constructor_pars_args as [[[] args]|] => //; cbn; destruct chop eqn:eqc; 
+  destruct (list_terms l1) using trev_ind => //; rewrite -TApp_TmkApps //.
+  eapply decompose_app_app in da. destruct l using rev_ind => //.
+  rewrite compile_terms_tappend // -TApp_TmkApps //.
+Qed.
+
+Lemma isFix_compile Σ f : 
+  ~~ EAstUtils.isFix f -> ~ isFix (compile Σ f).
+Proof.
+  move=> nf [] defs [n].
+  destruct f; simp_compile => /= //.
+  2:{ destruct p as [[] ?]; simp_compile => /= //.
+      destruct lookup_record_projs => /= //. }
+  rewrite compile_decompose.
+  destruct decompose_app eqn:da.
+  destruct construct_viewc.
+  destruct lookup_constructor_pars_args as [[[] args]|] => //; cbn; destruct chop eqn:eqc; 
+  destruct (list_terms l1) using trev_ind => //; rewrite -TApp_TmkApps //.
+  eapply decompose_app_app in da. destruct l using rev_ind => //.
+  rewrite compile_terms_tappend // -TApp_TmkApps //.
+Qed.
+
+Lemma isConstructApp_compile Σ f : 
+  ~~ EWcbvEval.isConstructApp f -> ~ isConstruct (compile Σ f).
+Proof.
+  move=> nf [] i [] n [] args.
+  destruct f; simp_compile => /= //.
+  2:{ destruct p as [[] ?]; simp_compile => /= //.
+      destruct lookup_record_projs => /= //. }
+  rewrite compile_decompose.
+  destruct decompose_app eqn:da.
+  destruct construct_viewc. 
+  { exfalso. rewrite (decompose_app_inv da) in nf.
+    rewrite EWcbvEval.isConstructApp_mkApps // in nf. }
+  eapply decompose_app_app in da. destruct l using rev_ind => //.
+  rewrite compile_terms_tappend // -TApp_TmkApps //.
+Qed.
+
+(* Lemma compile_tApp_etaexp Σ k f a :
+  wf_glob Σ ->
+  wellformed Σ k (tApp f a) ->
+  isEtaExp Σ f ->
+  isEtaExp Σ a ->
+  compile Σ (tApp f a) = TApp (compile Σ f) (compile Σ a).
+Proof.
+  intros wfΣ wf etaf etaa.
+  eapply compile_tApp; tea => //.
+  destruct decompose_app eqn:da.
+  destruct construct_viewc eqn:vc => //.
+  destruct lookup_constructor_pars_args as [[[] args']|] eqn:hl => // /=.
+  destruct chop eqn:eqc.
+  intros [Hl [Hf Ha]].
+  subst f.
+  move: etaf.
+  move/isEtaExp_mkApps => /=.
+  rewrite decompose_app_mkApps // /=.
+  move/andP => []. rewrite /isEtaExp_app hl. move/Nat.leb_le => /= etaind etal.
+  move: wf. rewrite -[tApp _ _](mkApps_app _ _ [a]).
+  rewrite wellformed_mkApps //.
+  move/andP=> [wfc wfargs].
+  eapply compile_mkApps_wf => //.
+  rewrite wellformed_mkApps //. erewrite wfc.
+  rewrite forallb_app in wfargs. now move/andP: wfargs.
+  simpl. rewrite hl.
+  rewrite PCUICTypeChecker.chop_firstn_skipn.
+  rewrite PCUICTypeChecker.chop_firstn_skipn in eqc. noconf eqc.
+  rewrite TApp_TmkApps.
+  f_equal. f_equal. rewrite {1}(remove_last_last l a Hl).
+  f_equal. rewrite map_app firstn_app. len. 
+  replace (args' - #|remove_last l|) with 0 by lia. cbn.
+  now rewrite app_nil_r.
+  rewrite {1}(remove_last_last l a Hl) map_app skipn_app.
+  rewrite list_terms_app. f_equal. len.
+  replace (args' - #|remove_last l|) with 0 by lia.
+  rewrite skipn_0 -Ha //.
+Qed. *)
+
+Lemma isEtaExp_tApp_nConstruct {Σ f a} : 
+  isEtaExp Σ (tApp f a) -> ~~ isConstructApp (tApp f a) -> isEtaExp Σ f && isEtaExp Σ a.
+Proof.
+  intros eta nc.
+  move/isEtaExp_tApp: eta.
+  destruct decompose_app eqn:da.
+  destruct construct_viewc. 
+  rewrite (decompose_app_inv da) in nc.
+  case/negP: nc. rewrite /isConstructApp decompose_app_mkApps //.
+  now move/and4P => [] _ _ -> ->.
+Qed.
+
+Lemma isConstructApp_tApp {f a} : EWcbvEval.isConstructApp (tApp f a) = EWcbvEval.isConstructApp f.
+Proof.
+  rewrite /EWcbvEval.isConstructApp. cbn.
+  now rewrite head_tApp.
+Qed.
+(* Lemma isConstruct_compile Σ k f : 
+  wf_glob Σ ->
+  wellformed Σ k f ->
+  isEtaExp Σ f ->
+  ~~ isConstructApp f -> ~ isConstruct (compile Σ f).
+Proof.
+  move=> wfΣ wf etaf nf [] ind [] n [] args.
+  destruct f; simp_compile => /= //.
+  2:{ destruct p as [[] ?]; simp_compile => /= //.
+      destruct lookup_record_projs => /= //. }
+  move/(isEtaExp_tApp_nConstruct etaf): nf => /andP[etaf1 etaf2].
+  rewrite (compile_tApp_etaexp k) //.
+Qed. *)
+
+From MetaCoq.Erasure Require Import EInduction ECSubst.
+
+Lemma compile_csubst Σ a k b : 
+  wf_glob Σ ->
+  (* wellformed Σ k a -> *)
+  (* wellformed Σ k b -> *)
+  compile Σ (ECSubst.csubst a k b) = instantiate (compile Σ a) k (compile Σ b).
+Proof.
+  intros wfΣ.
+  revert b k.
+  apply: MkAppsInd.rec. all:intros *. 
+  all:cbn; intros; simp_compile; cbn; try f_equal; eauto.
+
+  - destruct Nat.compare => //.
+  - rewrite csubst_mkApps.
+    eapply (compile_mkApps_wf (fun x => compile Σ (mkApps (csubst a k t) (map (csubst a k) u)) =
+    instantiate (compile Σ a) k x)); eauto. todo "wf".
+    destruct construct_viewc eqn:vc.
+    * destruct lookup_constructor_pars_args as [[pars args]|] eqn:hl => //.
+      destruct pars => //.
+      set (cargs := map _ u). simpl.
+      rewrite PCUICTypeChecker.chop_firstn_skipn.
+      specialize (H1 k).
+      cbn in H1.
+      eapply compile_mkApps_wf => //. todo "wf".
+      simpl. rewrite hl.
+      rewrite PCUICTypeChecker.chop_firstn_skipn.
+      rewrite !firstn_map instantiate_TConstruct. f_equal.
+      clear -X.
+      eapply (All_firstn (n:=args)) in X.
+      induction X => //.
+      cbn -[instantiates]. rewrite IHX //.
+      now rewrite p.
+    * eapply compile_mkApps => //. todo "wf".
+      
+
+
+Lemma WcbvEval_hom (fl := EWcbvEval.target_wcbv_flags) :
+  forall Σ, isEtaExp_env Σ -> wf_glob Σ ->
+  forall t t', 
+    wellformed Σ 0 t ->
+    isEtaExp Σ t -> 
+    EWcbvEval.eval Σ t t' ->
+    WcbvEval (compile_ctx Σ) (compile Σ t) (compile Σ t').
+Proof.
+  intros Σ etaΣ wfΣ.
+  eapply 
+    (EWcbvEvalEtaInd.eval_preserve_mkApps_ind fl Σ _ 
+      (wellformed Σ)) => //.
+  { intros. } (* eapply EWcbvEval.eval_wellformed. }*)
+  all:intros *.
+
+  - intros ev [IHev wfa wfb etaa etab].
+    intros ev' [IHev' wft wft' etat etat'].
+    eapply compile_tApp with (k := 0) => //. cbn; now rewrite wfa wft.
+    destruct decompose_app eqn:da.
+    simp_compile in IHev.
+    destruct (construct_viewc t0).
+    * destruct lookup_constructor_pars_args as [[[] args]|]=> // /=.
+      destruct chop eqn:eqch.
+      intros [Hl [ha ht]]. rewrite ha in ev.
+      eapply EWcbvEval.eval_construct' in ev as [? []]. solve_discr.
+    * econstructor; tea.
+  - intros ev [IHev wfa wfb etaa etab].
+    intros ev' [IHev' wft wft' etat etat'].
+    intros ev'' [IHev'' wfc wfr etac etar].
+    eapply compile_tApp with (k := 0) => //. cbn; now rewrite wfa wft.
+    simp_compile in IHev.
+    destruct decompose_app eqn:da.
+    destruct (construct_viewc t).
+    * destruct lookup_constructor_pars_args as [[[] args]|]=> // /=.
+      destruct chop eqn:eqch.
+      intros [Hl [ha ht]]. rewrite ha in ev.
+      eapply EWcbvEval.eval_construct' in ev as [? []]. solve_discr.
+    * econstructor; tea.
+      unfold whBetaStep.
+
+
+  - intros ev [IHev wfa wfb etaa etab] etab1.
+    intros ev' [IHev' wft wft' etat etat'].
+    simp_compile. econstructor; tea. admit.
+  - intros hbrs ev [IHev wfa wfb etaa etab].
+    intros isp hnth hskip hbr.
+    intros ev' [IHev' wft wft' etat etat'].
+    simp_compile.
+    rewrite compile_mkApps // /= in IHev. 
+    move: wfb; rewrite wellformed_mkApps // => /andP[] wfc wfargs.
+    destruct (wellformed_lookup_constructor_pars_args wfΣ wfc) as [nargs eq].
+    rewrite eq in IHev.
+    destruct chop eqn:eqc.
+    set (brs' := map _ brs). cbn.
+    assert (pars = 0).
+    { now eapply constructor_isprop_pars_decl_params in isp. }
+    subst pars. rewrite skipn_0 in hbr.
+    move: etab. rewrite EEtaExpanded.isEtaExp_mkApps_napp // /=.
+    move/andP => []. rewrite /isEtaExp_app /= eq /= => /Nat.leb_le hnargs hargs.
+
+    (* assert (l0 = nil) as ->. *)
+    (* { eapply eval_to_mkApps_Construct_inv in IHev. *)
+      (* destruct l0 => //. } *)
+    cbn in IHev. 
+    econstructor; tea.
+    rewrite PCUICTypeChecker.chop_firstn_skipn in eqc. noconf eqc.
+    (* eapply (f_equal (@List.length _)) in H. len in H. cbn in H. *)
+    (* rewrite skipn_length in H. assert (nargs = #|args|) by lia. *)
+    (* subst nargs. clear H hnargs. *)
+    (* rewrite firstn_all2. now len. *)
+    todo "subst".
+  - (* Fix case *) intros _.
+    rename f5 into f.
+    intros ev [IHev wff wffix etaf etafix].
+    intros unffix etafn eva [IHeva wfa wfav etaa etaav].
+    move=> evapp [IHevapp wftapp wfres etaapp etares].
+    move/isEtaExp_tApp.
+    eapply compile_tApp with (k := 0) => //.
+    { cbn; now rewrite wff wfa. }
+    destruct decompose_app eqn:da.
+    destruct construct_viewc eqn:vc.
+    * destruct lookup_constructor_pars_args as [[[] args]|]=> // /=.
+      destruct chop eqn:eqch.
+      intros [Hl [ha ht]]. rewrite ha in ev.
+      eapply EWcbvEval.eval_construct' in ev as [? []]. solve_discr.
+    * move=> /and4P[etat etal etaf' etaa'].
+      simp_compile in IHev.
+      set (mfix' := map _ mfix) in *.  
+      eapply (wAppFix (x := compile Σ fn)); tea.
+      { rewrite /mfix'. todo "whfix". }
+      move: IHevapp.
+      change (tApp fn av) with (mkApps fn [av]).
+      assert (isl : EAst.isLambda fn).
+      { move: etafix; cbn. simp_eta. intros hfix. 
+        unfold cunfold_fix in unffix. destruct nth_error eqn:hnth => //.
+        noconf unffix. eapply nth_error_forallb in hfix; tea. cbn in hfix.
+        move/andP: hfix => [] isl _.
+        eapply (isLambda_substl (fix_subst mfix)) in isl. 
+        destruct ECSubst.substl => //. }
+      destruct fn => //.
+      eapply compile_mkApps_wf; tea.
+      cbn. auto.
+  - (* No cofixpoints allowed *) 
+    intros cunfcof etafn etaargs.
+    move=> ev [IHev wfd wfcof wfdiscr etacof].
+    move: wfcof. rewrite wellformed_mkApps //.
+  - (* No cofixpoints allowed *) 
+    intros cunfcof etafn etaargs.
+    move=> ev [IHev wfd wfcof wfdiscr etacof].
+    move: wfcof. rewrite wellformed_mkApps //.
+  - (* Declarations *)
+    intros hdecl res hbod hev.
+    move => [] IHev wfbo wfr etab etares.
+    simp_compile. econstructor; tea. todo "lookups".
+  - move=> ev [IHev wfd wfcstr etad etacof] iisprop lenargs hnfh.
+    move=> ev' [IHev' wfarg wfres etaargs etares].
+    simp_compile.
+    destruct (lookup_record_projs) eqn:hl; simp_compile. cbn.
+    2:{ todo "wf projs". }
+    move: IHev.
+    unfold lookup_record_projs in hl.
+    destruct lookup_inductive as [[mdecl idecl]|] eqn:hl' => //. noconf hl.
+    eapply (compile_mkApps_wf) => // /=; tea.
+    destruct lookup_constructor_pars_args as [[[] args']|]=> // /=.
+    move: wfcstr; cbn. rewrite wellformed_mkApps //.
+    move=> /andP[] wfc wfargs. cbn -[lookup_constructor] in wfc.
+    unfold lookup_inductive in hl'.
+    destruct lookup_minductive eqn:hm => //.
+    pose proof (wellformed_lookup_inductive_pars _ wfΣ hm).
+    destruct chop eqn:eqch.
+    intros evd.
+    (* generalize (eval_to_mkApps_Construct_inv _ _ _ _ evd) => eql0. *)
+    (* destruct l0 => //. *)
+    rewrite PCUICTypeChecker.chop_firstn_skipn in eqch. noconf eqch.
+    (* eapply (f_equal (@List.length _)) in H0. rewrite skipn_length /= map_length in H0. *)
+    (* assert (args' >= #|args|). lia. cbn in evd. *)
+    (* rewrite firstn_all2 in evd. len. lia. *)
+    econstructor; tea. cbn. len. 
+    (* rewrite tlength_hom. *)
+    (* change (#|ind_projs idecl| =? #|args|) with (#|ind_projs idecl| == #|args|). *)
+    (* case: eqb_spec => lenargs. *)
+    (* { f_equal. assert (pars = 0). *)
+      (* admit. admit. } *)
+      admit.
+    (* { cbn in hl'. admit. } *)
+  - intros [hif' wff wff' etaf etaf'].
+    intros IHapp. intros nlam.
+    intros eva [iheva wfa wfa' etaa etaa'].
+    intros etaapp'.
+    eapply compile_tApp; tea. cbn. now erewrite wff, wfa.
+    destruct decompose_app eqn:da.
+    destruct construct_viewc eqn:vc.
+    * destruct lookup_constructor_pars_args as [[[] args']|] eqn:hl => // /=.
+      destruct chop eqn:hc.
+      intros [Hl [Hf11 Ha]].
+      change (tApp f' a') with (mkApps f' [a']).
+      clear IHapp. rewrite Hf11 in ev.
+      eapply EWcbvEval.eval_construct' in ev as [? []]. subst f'.
+      exfalso. move: nlam. rewrite !negb_or. rtoProp; intuition auto.
+      apply/negP: H0. rewrite negbK. unfold isConstructApp.
+      rewrite decompose_app_mkApps //.
+    * eapply (compile_tApp _ _ _ 0) => //. cbn. now rewrite wff' wfa'.
+      destruct (decompose_app (tApp f' a')) eqn:da'.
+      destruct (construct_viewc t0) eqn:vc'.
+      { destruct lookup_constructor_pars_args as [[[] args']|] eqn:hl => // /=.
+        pose proof (decompose_app_inv da').
+        eapply (f_equal EWcbvEval.isConstructApp) in H.
+        rewrite isConstructApp_tApp in H.
+        rewrite EWcbvEval.isConstructApp_mkApps /= /EWcbvEval.isConstructApp /= in H.
+        clear -nlam H. }
+      constructor; eauto.
+      rewrite !negb_or in nlam. rtoProp; intuition auto.
+      eapply (isLambda_compile Σ) in H. contradiction.
+      eapply (isFix_compile Σ) in H3; auto.
+      eapply (isConstructApp_compile Σ) in H3; auto.
+      eapply (isBox_compile Σ) in H1. contradiction.
+  - intros hl hargs evargs eta wfa wfa' IHargs.
+    eapply compile_mkApps_wf; eauto.
+    simpl. rewrite (lookup_constructor_pars_args_spec wfΣ hl).
+    rewrite PCUICTypeChecker.chop_firstn_skipn.
+    pose proof (wellformed_lookup_constructor_pars wfΣ hl).
+    rewrite firstn_all2. len. move: hargs; rewrite /EWcbvEval.cstr_arity => ->. lia.
+    rewrite H.
+    eapply compile_mkApps_wf; eauto.
+    simpl. rewrite (lookup_constructor_pars_args_spec wfΣ hl) H.
+    rewrite PCUICTypeChecker.chop_firstn_skipn.
+    rewrite firstn_all2. len. rewrite -(All2_length IHargs).
+    move: hargs; rewrite /EWcbvEval.cstr_arity => ->. lia.
+    constructor. clear -IHargs.
+    induction IHargs; cbn; constructor; intuition auto.
+    now destruct r.
+  - intros isat wf eta.
+    destruct t => //; simp_compile; econstructor. constructor.
+Qed.
+
 
 (*******************  broken from here  *****
 Lemma instantiate_hom:
   (forall bod n, L2d.term.WFTrm bod n -> 
-                 forall arg, strip (L2d.term.instantiate arg n bod) =
-                             instantiate (strip arg) n (strip bod)) /\
+                 forall arg, compile (L2d.term.instantiate arg n bod) =
+                             instantiate (compile arg) n (compile bod)) /\
   (forall bods n, L2d.term.WFTrms bods n ->
-                  forall arg, strips (L2d.term.instantiates arg n bods) =
-                              instantiates (strip arg) n (strips bods)) /\
+                  forall arg, compile_terms (L2d.term.instantiates arg n bods) =
+                              instantiates (compile arg) n (compile_terms bods)) /\
   (forall bods n, L2d.term.WFTrmBs bods n ->
-                  forall arg, stripBs (L2d.term.instantiateBrs arg n bods) =
-                              instantiateBrs (strip arg) n (stripBs bods)) /\
+                  forall arg, compileBs (L2d.term.instantiateBrs arg n bods) =
+                              instantiateBrs (compile arg) n (compileBs bods)) /\
   (forall ds n, L2d.term.WFTrmDs ds n  ->
-                forall arg, stripDs (L2d.term.instantiateDefs arg n ds) =
-                            instantiateDefs (strip arg) n (stripDs ds)).
+                forall arg, compile_defs (L2d.term.instantiateDefs arg n ds) =
+                            instantiateDefs (compile arg) n (compile_defs ds)).
 Proof.
   apply L2d.term.WFTrmTrmsBrsDefs_ind; intros;
     try (cbn; reflexivity); try (cbn; rewrite H0; reflexivity).
@@ -1379,41 +2115,41 @@ Proof.
   - cbn. rewrite H0. rewrite H2. reflexivity.
   - rewrite L2d.term.instantiate_TApp_mkApp.
     change
-      (strip (L2d.term.mkApp (L2d.term.instantiate arg n fn)
+      (compile (L2d.term.mkApp (L2d.term.instantiate arg n fn)
                             (L2d.compile.tcons
                                (L2d.term.instantiate arg n t)
                                (L2d.term.instantiates arg n ts))) =
-       instantiate (strip arg) n (strip (L2d.compile.TApp fn t ts))).
+       instantiate (compile arg) n (compile (L2d.compile.TApp fn t ts))).
     destruct (L2d.term.isConstruct_dec fn).
     + destruct i as [x0 [x1 [x2 [x3 jx]]]]. subst.
       unfold L2d.term.instantiate at 1.
       rewrite L2d.term.mkApp_goodFn; try not_isApp.
       change
-        (strip
+        (compile
            (L2d.compile.TApp (L2d.compile.TConstruct x0 x1 x2 x3)
                             (L2d.term.instantiate arg n t)
                             (L2d.term.instantiates arg n ts)) =
-         instantiate (strip arg) n
-                     (etaExp_cnstr x0 x1 x2 x3 (tcons (strip t) (strips ts)))).
+         instantiate (compile arg) n
+                     (etaExp_cnstr x0 x1 x2 x3 (tcons (compile t) (compile_terms ts)))).
       change
         (etaExp_cnstr x0 x1 x2 x3
-                      (tcons (strip (L2d.term.instantiate arg n t))
-                             (strips (L2d.term.instantiates arg n ts))) =
-         instantiate (strip arg) n
-                     (etaExp_cnstr x0 x1 x2 x3 (tcons (strip t) (strips ts)))).
+                      (tcons (compile (L2d.term.instantiate arg n t))
+                             (compile_terms (L2d.term.instantiates arg n ts))) =
+         instantiate (compile arg) n
+                     (etaExp_cnstr x0 x1 x2 x3 (tcons (compile t) (compile_terms ts)))).
       rewrite H3. rewrite H5.
       change
         (etaExp_cnstr x0 x1 x2 x3
-                      (instantiates (strip arg) n
-                                    (tcons (strip t) (strips ts))) =
-         instantiate (strip arg) n
-                     (etaExp_cnstr x0 x1 x2 x3 (tcons (strip t) (strips ts)))).
-      destruct (etaExp_cnstr_Sanity' x0 x1 x2 x3 (tcons (strip t) (strips ts))).
+                      (instantiates (compile arg) n
+                                    (tcons (compile t) (compile_terms ts))) =
+         instantiate (compile arg) n
+                     (etaExp_cnstr x0 x1 x2 x3 (tcons (compile t) (compile_terms ts)))).
+      destruct (etaExp_cnstr_Sanity' x0 x1 x2 x3 (tcons (compile t) (compile_terms ts))).
       * { rewrite H6.
           destruct (etaExp_cnstr_Sanity'
                       x0 x1 x2 x3 (instantiates
-                                     (strip arg) n (tcons (strip t)
-                                                          (strips ts)))).
+                                     (compile arg) n (tcons (compile t)
+                                                          (compile_terms ts)))).
           - rewrite H7.
          
 
@@ -1427,44 +2163,44 @@ Proof.
       * destruct i as [x0 [x1 [x2 [x3 jx]]]]. rewrite jx.
         change
           (etaExp_cnstr x0 x1 x2 x3
-                        (tcons (strip (L2d.term.instantiate arg n t))
-                               (strips (L2d.term.instantiates arg n ts))) =
-           instantiate (strip arg) n (strip (L2d.compile.TApp fn t ts))).
+                        (tcons (compile (L2d.term.instantiate arg n t))
+                               (compile_terms (L2d.term.instantiates arg n ts))) =
+           instantiate (compile arg) n (compile (L2d.compile.TApp fn t ts))).
         rewrite H3. rewrite H5.
         assert (k: fn = TConstruct x0 x1 tnil).
 
 
   (***************
   - destruct (L2d.term.isConstruct_dec t).
-    + change (strip (L2d.term.mkApp
+    + change (compile (L2d.term.mkApp
                        (L2d.term.instantiate arg n t)
                        (L2d.compile.tcons (L2d.term.instantiate arg n t0)
                                          (L2d.term.instantiates arg n t1))) =
-              instantiate (strip arg) n (strip (L2d.compile.TApp t t0 t1))).
+              instantiate (compile arg) n (compile (L2d.compile.TApp t t0 t1))).
       destruct i as [x0 [x1 [x2 [x3 jx]]]]. subst.
       rewrite L2d.term.mkApp_goodFn;
         [ | intros h; cbn in h; destruct h as [y0 [y1 [y2 jy]]]; discriminate].
       rewrite TAppCnstr_hom. unfold L2d.term.instantiate at 1.
       change
         (etaExp_cnstr x0 x1 x2 x3 
-                      (tcons (strip (L2d.term.instantiate arg n t0))
-                             (strips (L2d.term.instantiates arg n t1))) =
-         instantiate (strip arg) n
+                      (tcons (compile (L2d.term.instantiate arg n t0))
+                             (compile_terms (L2d.term.instantiates arg n t1))) =
+         instantiate (compile arg) n
                      (etaExp_cnstr x0 x1 x2 x3
-                                   (tcons (strip t0) (strips t1)))).
+                                   (tcons (compile t0) (compile_terms t1)))).
       rewrite H1. rewrite H0.
       change
         (etaExp_cnstr x0 x1 x2 x3
-                      (instantiates (strip arg) n
-                                    (tcons (strip t0) (strips t1))) =
-         instantiate (strip arg) n
+                      (instantiates (compile arg) n
+                                    (tcons (compile t0) (compile_terms t1))) =
+         instantiate (compile arg) n
                      (etaExp_cnstr x0 x1 x2 x3
-                                   (tcons (strip t0) (strips t1)))).
-      destruct (etaExp_spec x0 x1 x2 x3 (tcons (strip t0) (strips t1)))
+                                   (tcons (compile t0) (compile_terms t1)))).
+      destruct (etaExp_spec x0 x1 x2 x3 (tcons (compile t0) (compile_terms t1)))
         as [[j0 j1] | [j0 j1]];
       destruct  (etaExp_spec x0 x1 x2 x3
-                             (instantiates (strip arg) n
-                                           (tcons (strip t0) (strips t1))))
+                             (instantiates (compile arg) n
+                                           (tcons (compile t0) (compile_terms t1))))
         as [[k0 k1] | [k0 k1]];
       rewrite instantiates_pres_tlength in *; try contradiction.
       * cbn in H.
@@ -1474,8 +2210,8 @@ Proof.
         
         change
           (etaExp_cnstr x0 x1 x2 x3
-                        (instantiates (strip arg) n (tcons (strip t0) (strips t1))) =
-           instantiate (strip arg) n (TConstruct z0 z1 z2))
+                        (instantiates (compile arg) n (tcons (compile t0) (compile_terms t1))) =
+           instantiate (compile arg) n (TConstruct z0 z1 z2))
 
 
 
@@ -1483,13 +2219,13 @@ Proof.
    
     rewrite TApp_hom. 
     change
-      (strip (L2d.term.mkApp
+      (compile (L2d.term.mkApp
                 (L2d.term.instantiate arg n t)
                 (L2d.compile.tcons (L2d.term.instantiate arg n t0)
                                    (L2d.term.instantiates arg n t1))) =
-       (mkApp (instantiate (strip arg) n (strip t))
-              (tcons (instantiate (strip arg) n (strip t0))
-                     (instantiates (strip arg) n (strips t1))))).
+       (mkApp (instantiate (compile arg) n (compile t))
+              (tcons (instantiate (compile arg) n (compile t0))
+                     (instantiates (compile arg) n (compile_terms t1))))).
     rewrite <- H. rewrite <- H0. rewrite <- H1. 
     rewrite mkApp_hom. rewrite tcons_hom. reflexivity.
      ****************)
@@ -1498,39 +2234,39 @@ Proof.
     induction n0.
     + cbn.
     
-  - change (TCase p (strip (L2d.term.instantiate arg n t0))
-                  (stripDs (L2d.term.instantiateDefs arg n d)) =
-            (TCase p (instantiate (strip arg) n (strip t0))
-                   (instantiateDefs (strip arg) n (stripDs d)))).
+  - change (TCase p (compile (L2d.term.instantiate arg n t0))
+                  (compile_defs (L2d.term.instantiateDefs arg n d)) =
+            (TCase p (instantiate (compile arg) n (compile t0))
+                   (instantiateDefs (compile arg) n (compile_defs d)))).
     rewrite H0. rewrite H1. reflexivity.
-  - change (TFix (stripDs (L2d.term.instantiateDefs
+  - change (TFix (compile_defs (L2d.term.instantiateDefs
                              arg (n0 + L2d.compile.dlength d) d)) n =
             (TFix (instantiateDefs
-                     (strip arg) (n0 + dlength (stripDs d)) (stripDs d)) n)).
+                     (compile arg) (n0 + dlength (compile_defs d)) (compile_defs d)) n)).
     rewrite H. rewrite dlength_hom. reflexivity.
-  - change (tcons (strip (L2d.term.instantiate arg n t))
-                  (strips (L2d.term.instantiates arg n t0)) =
-            tcons (instantiate (strip arg) n (strip t))
-                  (instantiates (strip arg) n (strips t0))).
+  - change (tcons (compile (L2d.term.instantiate arg n t))
+                  (compile_terms (L2d.term.instantiates arg n t0)) =
+            tcons (instantiate (compile arg) n (compile t))
+                  (instantiates (compile arg) n (compile_terms t0))).
     rewrite H. rewrite H0. reflexivity.
-  - change (dcons n (strip (L2d.term.instantiate arg n1 t0)) n0
-                  (stripDs (L2d.term.instantiateDefs arg n1 d)) =
-            dcons n (instantiate (strip arg) n1 (strip t0)) n0
-                  (instantiateDefs (strip arg) n1 (stripDs d))).
+  - change (dcons n (compile (L2d.term.instantiate arg n1 t0)) n0
+                  (compile_defs (L2d.term.instantiateDefs arg n1 d)) =
+            dcons n (instantiate (compile arg) n1 (compile t0)) n0
+                  (instantiateDefs (compile arg) n1 (compile_defs d))).
     rewrite H0. rewrite H1. reflexivity.
 Qed.
  ****************************)
 
 (*****************  broken from here  ************
 Lemma instantiate_hom:
-  (forall bod arg n, strip (L2d.term.instantiate arg n bod) =
-                     instantiate (strip arg) n (strip bod)) /\
-  (forall bods arg n, strips (L2d.term.instantiates arg n bods) =
-                    instantiates (strip arg) n (strips bods)) /\
-  (forall bods arg n, stripBs (L2d.term.instantiateBrs arg n bods) =
-                    instantiateBrs (strip arg) n (stripBs bods)) /\
-  (forall ds arg n, stripDs (L2d.term.instantiateDefs arg n ds) =
-                    instantiateDefs (strip arg) n (stripDs ds)).
+  (forall bod arg n, compile (L2d.term.instantiate arg n bod) =
+                     instantiate (compile arg) n (compile bod)) /\
+  (forall bods arg n, compile_terms (L2d.term.instantiates arg n bods) =
+                    instantiates (compile arg) n (compile_terms bods)) /\
+  (forall bods arg n, compileBs (L2d.term.instantiateBrs arg n bods) =
+                    instantiateBrs (compile arg) n (compileBs bods)) /\
+  (forall ds arg n, compile_defs (L2d.term.instantiateDefs arg n ds) =
+                    instantiateDefs (compile arg) n (compile_defs ds)).
 Proof.
   apply L2d.compile.TrmTrmsBrsDefs_ind; intros; try (cbn; reflexivity);
     try (cbn; rewrite H; reflexivity).
@@ -1543,35 +2279,35 @@ Proof.
   - admit.
     (***************
   - destruct (L2d.term.isConstruct_dec t).
-    + change (strip (L2d.term.mkApp
+    + change (compile (L2d.term.mkApp
                        (L2d.term.instantiate arg n t)
                        (L2d.compile.tcons (L2d.term.instantiate arg n t0)
                                          (L2d.term.instantiates arg n t1))) =
-              instantiate (strip arg) n (strip (L2d.compile.TApp t t0 t1))).
+              instantiate (compile arg) n (compile (L2d.compile.TApp t t0 t1))).
       destruct i as [x0 [x1 [x2 [x3 jx]]]]. subst.
       rewrite L2d.term.mkApp_goodFn;
         [ | intros h; cbn in h; destruct h as [y0 [y1 [y2 jy]]]; discriminate].
       rewrite TAppCnstr_hom. unfold L2d.term.instantiate at 1.
       change
         (etaExp_cnstr x0 x1 x2 x3 
-                      (tcons (strip (L2d.term.instantiate arg n t0))
-                             (strips (L2d.term.instantiates arg n t1))) =
-         instantiate (strip arg) n
+                      (tcons (compile (L2d.term.instantiate arg n t0))
+                             (compile_terms (L2d.term.instantiates arg n t1))) =
+         instantiate (compile arg) n
                      (etaExp_cnstr x0 x1 x2 x3
-                                   (tcons (strip t0) (strips t1)))).
+                                   (tcons (compile t0) (compile_terms t1)))).
       rewrite H1. rewrite H0.
       change
         (etaExp_cnstr x0 x1 x2 x3
-                      (instantiates (strip arg) n
-                                    (tcons (strip t0) (strips t1))) =
-         instantiate (strip arg) n
+                      (instantiates (compile arg) n
+                                    (tcons (compile t0) (compile_terms t1))) =
+         instantiate (compile arg) n
                      (etaExp_cnstr x0 x1 x2 x3
-                                   (tcons (strip t0) (strips t1)))).
-      destruct (etaExp_spec x0 x1 x2 x3 (tcons (strip t0) (strips t1)))
+                                   (tcons (compile t0) (compile_terms t1)))).
+      destruct (etaExp_spec x0 x1 x2 x3 (tcons (compile t0) (compile_terms t1)))
         as [[j0 j1] | [j0 j1]];
       destruct  (etaExp_spec x0 x1 x2 x3
-                             (instantiates (strip arg) n
-                                           (tcons (strip t0) (strips t1))))
+                             (instantiates (compile arg) n
+                                           (tcons (compile t0) (compile_terms t1))))
         as [[k0 k1] | [k0 k1]];
       rewrite instantiates_pres_tlength in *; try contradiction.
       * cbn in H.
@@ -1581,8 +2317,8 @@ Proof.
         
         change
           (etaExp_cnstr x0 x1 x2 x3
-                        (instantiates (strip arg) n (tcons (strip t0) (strips t1))) =
-           instantiate (strip arg) n (TConstruct z0 z1 z2))
+                        (instantiates (compile arg) n (tcons (compile t0) (compile_terms t1))) =
+           instantiate (compile arg) n (TConstruct z0 z1 z2))
 
 
 
@@ -1590,13 +2326,13 @@ Proof.
    
     rewrite TApp_hom. 
     change
-      (strip (L2d.term.mkApp
+      (compile (L2d.term.mkApp
                 (L2d.term.instantiate arg n t)
                 (L2d.compile.tcons (L2d.term.instantiate arg n t0)
                                    (L2d.term.instantiates arg n t1))) =
-       (mkApp (instantiate (strip arg) n (strip t))
-              (tcons (instantiate (strip arg) n (strip t0))
-                     (instantiates (strip arg) n (strips t1))))).
+       (mkApp (instantiate (compile arg) n (compile t))
+              (tcons (instantiate (compile arg) n (compile t0))
+                     (instantiates (compile arg) n (compile_terms t1))))).
     rewrite <- H. rewrite <- H0. rewrite <- H1. 
     rewrite mkApp_hom. rewrite tcons_hom. reflexivity.
      ****************)
@@ -1605,33 +2341,33 @@ Proof.
     induction n0.
     + cbn.
     
-  - change (TCase p (strip (L2d.term.instantiate arg n t0))
-                  (stripDs (L2d.term.instantiateDefs arg n d)) =
-            (TCase p (instantiate (strip arg) n (strip t0))
-                   (instantiateDefs (strip arg) n (stripDs d)))).
+  - change (TCase p (compile (L2d.term.instantiate arg n t0))
+                  (compile_defs (L2d.term.instantiateDefs arg n d)) =
+            (TCase p (instantiate (compile arg) n (compile t0))
+                   (instantiateDefs (compile arg) n (compile_defs d)))).
     rewrite H0. rewrite H1. reflexivity.
-  - change (TFix (stripDs (L2d.term.instantiateDefs
+  - change (TFix (compile_defs (L2d.term.instantiateDefs
                              arg (n0 + L2d.compile.dlength d) d)) n =
             (TFix (instantiateDefs
-                     (strip arg) (n0 + dlength (stripDs d)) (stripDs d)) n)).
+                     (compile arg) (n0 + dlength (compile_defs d)) (compile_defs d)) n)).
     rewrite H. rewrite dlength_hom. reflexivity.
-  - change (tcons (strip (L2d.term.instantiate arg n t))
-                  (strips (L2d.term.instantiates arg n t0)) =
-            tcons (instantiate (strip arg) n (strip t))
-                  (instantiates (strip arg) n (strips t0))).
+  - change (tcons (compile (L2d.term.instantiate arg n t))
+                  (compile_terms (L2d.term.instantiates arg n t0)) =
+            tcons (instantiate (compile arg) n (compile t))
+                  (instantiates (compile arg) n (compile_terms t0))).
     rewrite H. rewrite H0. reflexivity.
-  - change (dcons n (strip (L2d.term.instantiate arg n1 t0)) n0
-                  (stripDs (L2d.term.instantiateDefs arg n1 d)) =
-            dcons n (instantiate (strip arg) n1 (strip t0)) n0
-                  (instantiateDefs (strip arg) n1 (stripDs d))).
+  - change (dcons n (compile (L2d.term.instantiate arg n1 t0)) n0
+                  (compile_defs (L2d.term.instantiateDefs arg n1 d)) =
+            dcons n (instantiate (compile arg) n1 (compile t0)) n0
+                  (instantiateDefs (compile arg) n1 (compile_defs d))).
     rewrite H0. rewrite H1. reflexivity.
 Qed.
   
 Lemma whBetaStep_hom:
   forall bod arg args,
     L2d.term.WFTrm bod 0 ->
-    strip (L2d.term.whBetaStep bod arg args) =
-    whBetaStep (strip bod) (strip arg) (strips args).
+    compile (L2d.term.whBetaStep bod arg args) =
+    whBetaStep (compile bod) (compile arg) (compile_terms args).
 Proof.
   intros bod arg args h.
   unfold L2d.term.whBetaStep, whBetaStep.
@@ -1642,27 +2378,27 @@ Proof.
     destruct (L2d.term.isApp_dec (L2d.term.instantiate arg 0 bod)).
     + destruct i as [x0 [x1 [x2 jx]]]. rewrite jx. clear jx.
     change
-      (strip (L2d.compile.TApp
+      (compile (L2d.compile.TApp
                 x0 x1 (L2d.term.tappend x2 (L2d.compile.tcons t args))) =
-       mkApp (strip (L2d.compile.TApp x0 x1 x2))
-             (strips (L2d.compile.tcons t args))).
+       mkApp (compile (L2d.compile.TApp x0 x1 x2))
+             (compile_terms (L2d.compile.tcons t args))).
     destruct (L2d.term.isConstruct_dec x0).
       * { destruct i as [i0 [i1 [i2 [i3 ji]]]]. subst.
         change
           (etaExp_cnstr i0 i1 i2 i3
-                        (tcons (strip x1)
-                               (strips (L2d.term.tappend
+                        (tcons (compile x1)
+                               (compile_terms (L2d.term.tappend
                                           x2 (L2d.compile.tcons t args)))) =
            mkApp (etaExp_cnstr i0 i1 i2 i3
-                        (tcons (strip x1) (strips x2)))
-                 (strips (L2d.compile.tcons t args))).
-        rewrite strips_tappend. rewrite tcons_hom.   
+                        (tcons (compile x1) (compile_terms x2)))
+                 (compile_terms (L2d.compile.tcons t args))).
+        rewrite compile_terms_tappend. rewrite tcons_hom.   
         destruct (etaExp_cnstr_Sanity' i0 i1 i2 i3
-                                        (tcons (strip x1) (strips x2))).
+                                        (tcons (compile x1) (compile_terms x2))).
           - rewrite H. rewrite mkApp_goodFn; try not_isApp.
         destruct (etaExp_cnstr_Sanity' i0 i1 i2 i3
-                                         (tcons (strip x1)
-                                                (compile.tappend (strips x2) (tcons (strip t) (strips args))))).
+                                         (tcons (compile x1)
+                                                (compile.tappend (compile_terms x2) (tcons (compile t) (compile_terms args))))).
         rewrite H0.
 
         rewrite <- (proj1 instantiate_hom); try assumption.
@@ -1670,14 +2406,14 @@ Proof.
     + destruct i as [y0 [y1 [y2 [y3 jy]]]]. subst.
       change
         (etaExp_cnstr y0 y1 y2 y3
-                      (tcons (strip x1) (strips (L2d.term.tappend x2 args))) =
+                      (tcons (compile x1) (compile_terms (L2d.term.tappend x2 args))) =
          mkApp (etaExp_cnstr y0 y1 y2 y3
-                             (tcons (strip x1) (strips x2)))
-               (strips args)).
+                             (tcons (compile x1) (compile_terms x2)))
+               (compile_terms args)).
       destruct (etaExp_cnstr_Sanity'
                   y0 y1 y2 y3
-                  (tcons (strip x1) (strips (L2d.term.tappend x2 args)))),
-      (etaExp_cnstr_Sanity'  y0 y1 y2 y3 (tcons (strip x1) (strips x2)));
+                  (tcons (compile x1) (compile_terms (L2d.term.tappend x2 args)))),
+      (etaExp_cnstr_Sanity'  y0 y1 y2 y3 (tcons (compile x1) (compile_terms x2)));
         rewrite H; rewrite H0.
       * { cbn. destruct args. cbn.
           - apply f_equal3; try reflexivity.
@@ -1694,12 +2430,12 @@ Proof.
       apply (proj1 instantiate_hom). assumption.
     + rewrite L2d.term.mkApp_goodFn; try assumption.
       change
-        (strip (L2d.compile.TApp (L2d.term.instantiate arg 0 bod) t args) =
-         mkApp (instantiate (strip arg) 0 (strip bod))
-               (tcons (strip t) (strips args))).
+        (compile (L2d.compile.TApp (L2d.term.instantiate arg 0 bod) t args) =
+         mkApp (instantiate (compile arg) 0 (compile bod))
+               (tcons (compile t) (compile_terms args))).
       rewrite mkApp_goodFn.
       * admit.        
-      * intros k. elim n. apply strip_pres_isApp.
+      * intros k. elim n. apply compile_pres_isApp.
         rewrite (proj1 instantiate_hom); assumption.       
 Qed.
 
@@ -1713,16 +2449,16 @@ Qed.
 (***
 Lemma TConstruct_hom:
   forall i n args,
-    strip (L2d.compile.TConstruct i n args) = TConstruct i n args.
+    compile (L2d.compile.TConstruct i n args) = TConstruct i n args.
 intros. simpl.  destruct i. reflexivity.
 Qed.
 ***)
 
-Lemma optStrip_match:
+Lemma optcompile_match:
   forall x (f:L2Term -> L2Term) (g:Term -> Term), 
-    (forall z, strip (f z) = g (strip z)) ->
-    optStrip (match x with Some y => Some (f y) | None => None end) =
-    match (optStrip x) with Some y => Some (g y) | None => None end.
+    (forall z, compile (f z) = g (compile z)) ->
+    optcompile (match x with Some y => Some (f y) | None => None end) =
+    match (optcompile x) with Some y => Some (g y) | None => None end.
 induction x; intros f g h; simpl.
 - rewrite h; reflexivity.
 - reflexivity.
@@ -1730,8 +2466,8 @@ Qed.
 
 Lemma whCaseStep_hom:
   forall n brs ts,
-    optStrip (L2d.term.whCaseStep n ts brs) =
-    whCaseStep n (strips ts) (stripDs brs).
+    optcompile (L2d.term.whCaseStep n ts brs) =
+    whCaseStep n (compile_terms ts) (compile_defs brs).
 destruct n, brs; intros; simpl; try reflexivity.
 - unfold whCaseStep. simpl. rewrite mkApp_hom. reflexivity.
 - unfold whCaseStep. unfold L2d.term.whCaseStep. cbn. 
@@ -1741,36 +2477,36 @@ destruct n, brs; intros; simpl; try reflexivity.
 Qed.
 
 Lemma TFix_hom:
-  forall defs n, strip (L2d.compile.TFix defs n) = TFix (stripDs defs) n.
+  forall defs n, compile (L2d.compile.TFix defs n) = TFix (compile_defs defs) n.
 reflexivity.
 Qed.
 
 Lemma TProd_hom:
   forall nm ty bod,
-    strip (L2d.compile.TProd nm ty bod) = TProd nm (strip bod).
+    compile (L2d.compile.TProd nm ty bod) = TProd nm (compile bod).
 reflexivity.
 Qed.
 
 
 Lemma TLetIn_hom:
   forall nm dfn ty bod,
-    strip (L2d.compile.TLetIn nm dfn ty bod) =
-    TLetIn nm (strip dfn) (strip bod).
+    compile (L2d.compile.TLetIn nm dfn ty bod) =
+    TLetIn nm (compile dfn) (compile bod).
 reflexivity.
 Qed.
 
 Lemma TCase_hom:
   forall n ty mch brs,
-    strip (L2d.compile.TCase n ty mch brs) =
-    TCase n (strip mch) (stripDs brs).
+    compile (L2d.compile.TCase n ty mch brs) =
+    TCase n (compile mch) (compile_defs brs).
 reflexivity.
 Qed.
 
 Lemma fold_left_hom:
 forall (F:L2Term -> nat -> L2Term) 
-       (stripF:Term -> nat -> Term) (ns:list nat) (t:L2Term),
-  (forall (s:L2Term) (n:nat), strip (F s n) = stripF (strip s) n) ->
-  strip (fold_left F ns t) = fold_left stripF ns (strip t).
+       (compileF:Term -> nat -> Term) (ns:list nat) (t:L2Term),
+  (forall (s:L2Term) (n:nat), compile (F s n) = compileF (compile s) n) ->
+  compile (fold_left F ns t) = fold_left compileF ns (compile t).
 induction ns; intros t h.
 - intuition.
 - simpl. rewrite IHns.
@@ -1780,15 +2516,15 @@ Qed.
 
 Lemma pre_whFixStep_hom:
   forall body dts args,
-    pre_whFixStep (strip body) (stripDs dts) (strips args) =
-    strip (L2d.term.pre_whFixStep body dts args).
+    pre_whFixStep (compile body) (compile_defs dts) (compile_terms args) =
+    compile (L2d.term.pre_whFixStep body dts args).
 Proof.
   intros body dts args.
   destruct dts, args; unfold pre_whFixStep, L2d.term.pre_whFixStep;
   simpl; rewrite mkApp_hom; try reflexivity.
   - rewrite (fold_left_hom _
           (fun (bod : Term) (ndx : nat) =>
-                instantiate (TFix (dcons n (strip t0) n0 (stripDs dts)) ndx)
+                instantiate (TFix (dcons n (compile t0) n0 (compile_defs dts)) ndx)
                   0 bod)).
     + rewrite <- (dcons_hom _ L2d.compile.prop).
       rewrite (proj1 instantiate_hom).
@@ -1796,7 +2532,7 @@ Proof.
     + intros. rewrite (proj1 instantiate_hom). simpl. reflexivity.
   - rewrite (fold_left_hom _
             (fun (bod : Term) (ndx : nat) =>
-         instantiate (TFix (dcons n (strip t0) n0 (stripDs dts)) ndx) 0 bod)).
+         instantiate (TFix (dcons n (compile t0) n0 (compile_defs dts)) ndx) 0 bod)).
     + rewrite dlength_hom. rewrite (proj1 instantiate_hom).
       rewrite tcons_hom. reflexivity.
     + intros. rewrite (proj1 instantiate_hom).
@@ -1805,43 +2541,43 @@ Qed.
 
 Lemma tsplit_hom:
   forall ix arg args,
-    optStrip_split (L2d.term.tsplit ix arg args) =
-    tsplit ix (strip arg) (strips args).
+    optcompile_split (L2d.term.tsplit ix arg args) =
+    tsplit ix (compile arg) (compile_terms args).
 Proof.
   intros ix arg args.
   functional induction (L2d.term.tsplit ix arg args); cbn; intros.
   - reflexivity.
   - destruct n. elim y. reflexivity.
   - destruct ls; cbn; reflexivity.
-  - case_eq (tsplit m (strip t) (strips ts)); intros.
+  - case_eq (tsplit m (compile t) (compile_terms ts)); intros.
     + destruct s.
       assert (j0:= L2d.term.tsplit_sanity m t ts). rewrite e1 in j0.
-      assert (j1:= tsplit_sanity m (strip t) (strips ts)).
+      assert (j1:= tsplit_sanity m (compile t) (compile_terms ts)).
       rewrite H in j1. destruct j1.
-      assert (j2: tlength (strips ts) = tlength fsts + tlength lsts).
+      assert (j2: tlength (compile_terms ts) = tlength fsts + tlength lsts).
       { apply (f_equal tlength) in H0. rewrite tlength_tappend in H0.
         cbn in H0. omega. }
       rewrite tlength_hom in j2. rewrite j2 in j0. rewrite H1 in j0. omega.
     + reflexivity.
-  - destruct (tsplit m (strip t) (strips ts)).
-    + destruct s0. rewrite e1 in IHo. rewrite optStrip_split_hom in IHo.
+  - destruct (tsplit m (compile t) (compile_terms ts)).
+    + destruct s0. rewrite e1 in IHo. rewrite optcompile_split_hom in IHo.
       myInjection IHo. reflexivity.
-    + rewrite e1 in IHo.  rewrite optStrip_split_hom in IHo.
+    + rewrite e1 in IHo.  rewrite optcompile_split_hom in IHo.
       discriminate.
 Qed.
 
-Lemma optStripCanP_hom':
-  forall z, optStripCanP (Some z) =
-            Some (fst (fst z), strips (snd (fst z)), snd z).
+Lemma optcompileCanP_hom':
+  forall z, optcompileCanP (Some z) =
+            Some (fst (fst z), compile_terms (snd (fst z)), snd z).
 intros. destruct z as [[z0 z1] z2]. cbn. reflexivity.
 Qed.
 
 Lemma WcbvEval_hom:
   forall p,
     (forall t t', L2d.wcbvEval.WcbvEval p t t' ->
-                  WcbvEval (stripEnv p) (strip t) (strip t')) /\
+                  WcbvEval (compile_ctx Σ) (compile t) (compile t')) /\
     (forall ts ts', L2d.wcbvEval.WcbvEvals p ts ts' ->
-                    WcbvEvals (stripEnv p) (strips ts) (strips ts')).
+                    WcbvEvals (compile_ctx Σ) (compile_terms ts) (compile_terms ts')).
 Proof.
   intros p.
   apply L2d.wcbvEval.WcbvEvalEvals_ind; intros; try reflexivity;
@@ -1883,150 +2619,150 @@ Print Assumptions WcbvEval_hom.
 (** WcbvEval_hom is nice, but it is stronger than necessary to prove 
 *** certiL2_to_L2Correct (in instances.v).
 **)
-Corollary strip_pres_eval:
+Corollary compile_pres_eval:
   forall (p:environ L2d.compile.Term) (t tv:L2d.compile.Term),
     L2d.wcbvEval.WcbvEval p t tv ->
-    exists stv, WcbvEval (stripEnv p) (strip t) stv.
+    exists stv, WcbvEval (compile_ctx Σ) (compile t) stv.
 Proof.
-  intros. exists (strip tv). apply (proj1 (WcbvEval_hom _)).
+  intros. exists (compile tv). apply (proj1 (WcbvEval_hom _)).
   assumption.
 Qed.
 
 Corollary wcbvEval_hom:
   forall p n t t',
     L2d.wcbvEval.wcbvEval p n t = Ret t' ->
-    exists m, wcbvEval (stripEnv p) m (strip t) = Ret (strip t').
+    exists m, wcbvEval (compile_ctx Σ) m (compile t) = Ret (compile t').
 Proof.
   intros. 
   assert (j1:= proj1 (L2d.wcbvEval.wcbvEval_WcbvEval p n) _ _ H).
   assert (k0:= proj1 (WcbvEval_hom p) _ _ j1).
-  assert (j2:= @WcbvEval_wcbvEval (stripEnv p) (strip t) (strip t') k0).
+  assert (j2:= @WcbvEval_wcbvEval (compile_ctx Σ) (compile t) (compile t') k0).
   destruct j2 as [ny jny].
   exists ny. eapply jny. omega.
 Qed.
 
 
-Lemma Prf_strip_inv:
-  forall s st, TProof st = strip s ->
-              exists t, s = L2d.compile.TProof t /\ st = strip t.
+Lemma Prf_compile_inv:
+  forall s st, TProof st = compile s ->
+              exists t, s = L2d.compile.TProof t /\ st = compile t.
 Proof.
   destruct s; simpl; intros h; try discriminate.
   intros. myInjection H. exists s. intuition.
 Qed.
   
-Lemma Lam_strip_inv:
-  forall nm bod s, TLambda nm bod = strip s ->
+Lemma Lam_compile_inv:
+  forall nm bod s, TLambda nm bod = compile s ->
    exists sty sbod, 
-     (L2d.compile.TLambda nm sty sbod) = s /\ bod = strip sbod.
+     (L2d.compile.TLambda nm sty sbod) = s /\ bod = compile sbod.
 Proof.
   intros nm bod; destruct s; simpl; intros h; try discriminate.
   - myInjection h. exists s1, s2. intuition. 
 Qed.
 
-Lemma Prod_strip_inv:
-  forall nm bod s, TProd nm bod = strip s ->
+Lemma Prod_compile_inv:
+  forall nm bod s, TProd nm bod = compile s ->
    exists sty sbod, 
-     (L2d.compile.TProd nm sty sbod) = s /\ bod = strip sbod.
+     (L2d.compile.TProd nm sty sbod) = s /\ bod = compile sbod.
 Proof.
   intros nm bod; destruct s; simpl; intros h; try discriminate.
   - myInjection h. exists s1, s2. intuition. 
 Qed.
 
-Lemma Cast_strip_inv:
-  forall tm s, TCast tm = strip s ->
+Lemma Cast_compile_inv:
+  forall tm s, TCast tm = compile s ->
    exists stm sty, 
-     (L2d.compile.TCast stm sty) = s /\ tm = strip stm.
+     (L2d.compile.TCast stm sty) = s /\ tm = compile stm.
 Proof.
   intros tm; destruct s; simpl; intros h; try discriminate.
   - myInjection h. exists s1, s2. intuition. 
 Qed.
 
-Lemma Construct_strip_inv:
+Lemma Construct_compile_inv:
   forall i n arty s,
-    TConstruct i n arty = strip s -> L2d.compile.TConstruct i n arty = s.
+    TConstruct i n arty = compile s -> L2d.compile.TConstruct i n arty = s.
 Proof.
   intros i n. destruct s; simpl; intros h; try discriminate.
   - myInjection h. reflexivity.
 Qed.
 
-Lemma Sort_strip_inv:
-  forall srt s, TSort srt = strip s -> L2d.compile.TSort srt = s.
+Lemma Sort_compile_inv:
+  forall srt s, TSort srt = compile s -> L2d.compile.TSort srt = s.
 Proof.
   intros srt. destruct s; simpl; intros h; try discriminate.
   - myInjection h. reflexivity.
 Qed.
 
-Lemma Ind_strip_inv:
-  forall i s, TInd i = strip s -> L2d.compile.TInd i = s.
+Lemma Ind_compile_inv:
+  forall i s, TInd i = compile s -> L2d.compile.TInd i = s.
 Proof.
   intros i. destruct s; simpl; intros h; try discriminate.
   - myInjection h. reflexivity.
 Qed.
 
-Lemma Const_strip_inv:
-  forall nm s, TConst nm = strip s -> L2d.compile.TConst nm = s.
+Lemma Const_compile_inv:
+  forall nm s, TConst nm = compile s -> L2d.compile.TConst nm = s.
 Proof.
   intros nm. destruct s; simpl; intros h; try discriminate.
   - myInjection h. reflexivity.
 Qed.
 
-Lemma Fix_strip_inv:
-  forall ds n s, TFix ds n = strip s ->
-    exists sds, (L2d.compile.TFix sds n) = s /\ ds = stripDs sds.
+Lemma Fix_compile_inv:
+  forall ds n s, TFix ds n = compile s ->
+    exists sds, (L2d.compile.TFix sds n) = s /\ ds = compile_defs sds.
 Proof.
   intros ds n. destruct s; simpl; intros h; try discriminate.
   - myInjection h. exists d. intuition.
 Qed.
 
-Lemma App_strip_inv:
-  forall fn arg args s, TApp fn arg args = strip s ->
+Lemma App_compile_inv:
+  forall fn arg args s, TApp fn arg args = compile s ->
     exists sfn sarg sargs,
       (L2d.compile.TApp sfn sarg sargs) = s /\
-      fn = strip sfn /\ arg = strip sarg /\ args = strips sargs.
+      fn = compile sfn /\ arg = compile sarg /\ args = compile_terms sargs.
 Proof.
   intros fn arg args. destruct s; simpl; intros h; try discriminate.
   - myInjection h. exists s1, s2, t. intuition.
 Qed.
 
-Lemma LetIn_strip_inv:
-  forall nm dfn bod s, TLetIn nm dfn bod = strip s ->
+Lemma LetIn_compile_inv:
+  forall nm dfn bod s, TLetIn nm dfn bod = compile s ->
     exists sdfn sty sbod,
       (L2d.compile.TLetIn nm sdfn sty sbod = s) /\
-      dfn = strip sdfn /\ bod = strip sbod.
+      dfn = compile sdfn /\ bod = compile sbod.
 Proof.
   intros nm dfn bod s. destruct s; simpl; intros h; try discriminate.
   - myInjection h. exists s1, s2, s3. intuition.
 Qed.
 
-Lemma Case_strip_inv:
-  forall m mch brs s, TCase m mch brs = strip s ->
+Lemma Case_compile_inv:
+  forall m mch brs s, TCase m mch brs = compile s ->
     exists sty smch sbrs, (L2d.compile.TCase m sty smch sbrs = s) /\
-              mch = strip smch /\ brs = stripDs sbrs.
+              mch = compile smch /\ brs = compile_defs sbrs.
 Proof.
   intros m mch brs s. destruct s; simpl; intros h; try discriminate.
   - myInjection h. exists s1, s2, d. intuition.
 Qed.
 
-Lemma tnil_strip_inv:
-  forall ts, tnil = strips ts -> ts = L2d.compile.tnil.
+Lemma tnil_compile_inv:
+  forall ts, tnil = compile_terms ts -> ts = L2d.compile.tnil.
 Proof.
   induction ts; intros; try reflexivity.
   - simpl in H. discriminate.
 Qed.
 
-Lemma tcons_strip_inv:
-  forall t ts us, tcons t ts = strips us ->
+Lemma tcons_compile_inv:
+  forall t ts us, tcons t ts = compile_terms us ->
     exists st sts, (L2d.compile.tcons st sts = us) /\ 
-                   t = strip st /\ ts = strips sts.
+                   t = compile st /\ ts = compile_terms sts.
 Proof.
   intros t ts us. destruct us; simpl; intros h; try discriminate.
   - myInjection h. exists t0, us. intuition.
 Qed.
 
-Lemma dcons_strip_inv:
-  forall nm t m ts us, dcons nm t m ts = stripDs us ->
+Lemma dcons_compile_inv:
+  forall nm t m ts us, dcons nm t m ts = compile_defs us ->
     exists ty st sts, (L2d.compile.dcons nm ty st m sts = us) /\ 
-                   t = strip st /\ ts = stripDs sts.
+                   t = compile st /\ ts = compile_defs sts.
 Proof.
   intros nm t m ts us. destruct us; simpl; intros h; try discriminate.
   - myInjection h. exists t0, t1, us. intuition.
@@ -2035,23 +2771,23 @@ Qed.
 Lemma whCaseStep_Hom:
   forall n ts bs t,
     L2d.term.whCaseStep n ts bs = Some t -> 
-    whCaseStep n (strips ts) (stripDs bs) = Some (strip t).
+    whCaseStep n (compile_terms ts) (compile_defs bs) = Some (compile t).
 Proof.
-  intros n ts bs t h. rewrite <- whCaseStep_hom. rewrite <- optStrip_hom.
+  intros n ts bs t h. rewrite <- whCaseStep_hom. rewrite <- optcompile_hom.
   apply f_equal. assumption.
 Qed.
 
-Definition excStrip (t:exception L2Term) : exception Term :=
+Definition exccompile (t:exception L2Term) : exception Term :=
   match t with
     | Exc str => Exc str
-    | Ret t => Ret (strip t)
+    | Ret t => Ret (compile t)
   end.
 
 
 Theorem L2WcbvEval_sound_for_L2WcbvEval:
   forall (p:environ L2d.compile.Term) (t:L2d.compile.Term) (L2s:Term),
-    WcbvEval (stripEnv p) (strip t) L2s ->
-  forall s, L2d.wcbvEval.WcbvEval p t s -> L2s = strip s.
+    WcbvEval (compile_ctx Σ) (compile t) L2s ->
+  forall s, L2d.wcbvEval.WcbvEval p t s -> L2s = compile s.
 Proof.
   intros. refine (WcbvEval_single_valued _ _).
   - eassumption.
@@ -2063,21 +2799,21 @@ Print Assumptions L2WcbvEval_sound_for_L2WcbvEval.
 Lemma sound_and_complete:
   forall (p:environ L2d.compile.Term) (t s:L2d.compile.Term),
     L2d.wcbvEval.WcbvEval p t s ->
-    WcbvEval (stripEnv p) (strip t) (strip s).
+    WcbvEval (compile_ctx Σ) (compile t) (compile s).
 Proof.
   intros p t s h. apply (proj1 (WcbvEval_hom p)). assumption.
 Qed.
 
 Lemma sac_complete:
   forall p t s, L2d.wcbvEval.WcbvEval p t s ->
-                WcbvEval (stripEnv p) (strip t) (strip s).
+                WcbvEval (compile_ctx Σ) (compile t) (compile s).
 Proof.
   intros. apply sound_and_complete. assumption.
 Qed.
 
 Lemma sac_sound:
   forall p t s, L2d.wcbvEval.WcbvEval p t s ->
-  forall L2s, WcbvEval (stripEnv p) (strip t) L2s -> L2s = strip s.
+  forall L2s, WcbvEval (compile_ctx Σ) (compile t) L2s -> L2s = compile s.
 Proof.
   intros p t s h1 L2s h2.
   apply (WcbvEval_single_valued h2). apply (sound_and_complete h1).
